NAND_Femto.thy
@@ -141,4 +141,1658 @@ value "get_trans (functional_simulate 10 nand) 1 C"
 
 value "signal_of (functional_simulate 10 nand) C 100"
 
+value [code] "to_signal (to_transaction2 (empty_trans :: nat \<Rightarrow>\<^sub>0 sig \<rightharpoonup> bool)) A 123456"
+
+definition nand2 :: "sig conc_stmt" where
+  "nand2 = process {A, B} : Bcomp
+                            (Bassign_trans C (Bnand (Bsig A) (Bsig B)) 1)
+                            (Bassign_trans A (Bnand (Bsig A) (Bsig B)) 3)"
+
+definition "test_trans = Pm_fmap (fmap_of_list [(4::nat, [A \<mapsto> True, B \<mapsto> True])])"
+definition  "test2 = functional_simulate_fin 2 0 def_state {A, B, C} 0 nand2 test_trans"
+
+value [code] "to_transaction2 test2 C"
+
+definition nand3 :: "sig conc_stmt" where
+  "nand3 = process {A, B} : Bassign_trans C (Bnand (Bsig A) (Bsig B)) 1"
+
+\<comment> \<open>Specific lemmas about @{term "nand"} and @{term "nand3"}\<close>
+
+lemma nand_does_not_modify_AB:
+  assumes "b_seq_exec t \<sigma> \<gamma> \<theta> (get_seq nand) \<tau> = \<tau>'"
+  shows "\<And>i. i \<ge> t \<Longrightarrow> s \<noteq> C \<Longrightarrow> lookup \<tau> i s = lookup \<tau>' i s"
+  using b_seq_exec_modifies_local assms unfolding nand_def
+  by (metis conc_stmt.sel(4) empty_set list.simps(15) signals_in.simps(3) singletonD)
+
+lemma nand3_does_not_modify_AB:
+  assumes "b_seq_exec t \<sigma> \<gamma> \<theta> (get_seq nand3) \<tau> = \<tau>'"
+  shows "\<And>i. i \<ge> t \<Longrightarrow> s \<noteq> C \<Longrightarrow> lookup \<tau> i s = lookup \<tau>' i s"
+  using b_seq_exec_modifies_local assms unfolding nand3_def
+  by (metis conc_stmt.sel(4) empty_set list.simps(15) signals_in.simps(2) singletonD)
+
+lemma nand_does_not_modify_AB':
+  assumes "\<And>n. n < t \<Longrightarrow> lookup \<tau> n = 0"
+  assumes "b_seq_exec t \<sigma> \<gamma> \<theta> (get_seq nand) \<tau> = \<tau>'"
+  shows "\<And>i. s \<noteq> C \<Longrightarrow> lookup \<tau> i s = lookup \<tau>' i s"
+  using assms unfolding nand_def
+  by (metis assms(2) b_seq_exec_preserve_trans_removal nand_does_not_modify_AB not_le)
+
+lemma nand3_does_not_modify_AB':
+  assumes "\<And>n. n < t \<Longrightarrow> lookup \<tau> n = 0"
+  assumes "b_seq_exec t \<sigma> \<gamma> \<theta> (get_seq nand3) \<tau> = \<tau>'"
+  shows "\<And>i. s \<noteq> C \<Longrightarrow> lookup \<tau> i s = lookup \<tau>' i s"
+  using assms unfolding nand3_def
+  by (metis assms(2) b_seq_exec_preserve_trans_removal nand3_does_not_modify_AB not_le)
+
+lemma seq_nand_does_not_modify_signals_AB:
+  assumes "\<And>n. n < t \<Longrightarrow> lookup \<tau> n = 0"
+  assumes "b_seq_exec t \<sigma> \<gamma> \<theta> (get_seq nand) \<tau> = \<tau>'"
+  assumes "s \<noteq> C"
+  shows "\<And>i. signal_of \<tau> s i = signal_of \<tau>' s i"
+  using b_seq_does_not_modify_signals[OF assms(1-2)] assms(3) unfolding nand_def
+  by auto
+
+lemma seq_nand3_does_not_modify_signals_AB:
+  assumes "\<And>n. n < t \<Longrightarrow> lookup \<tau> n = 0"
+  assumes "b_seq_exec t \<sigma> \<gamma> \<theta> (get_seq nand3) \<tau> = \<tau>'"
+  assumes "s \<noteq> C"
+  shows "\<And>i. signal_of \<tau> s i = signal_of \<tau>' s i"
+  using b_seq_does_not_modify_signals[OF assms(1-2)] assms(3) unfolding nand3_def
+  by auto
+
+lemma nand_does_not_modify_signals_AB:
+  assumes "\<And>n. n < t \<Longrightarrow> lookup \<tau> n = 0"
+  assumes "b_conc_exec t \<sigma> \<gamma> \<theta> nand \<tau> = \<tau>'"
+  assumes "s \<noteq> C"
+  shows "\<And>i. signal_of \<tau> s i = signal_of \<tau>' s i"
+  using b_conc_exec_does_not_modify_signals[OF assms(1-2)] assms(3)
+  unfolding nand_def by auto
+
+lemma nand3_does_not_modify_signals_AB:
+  assumes "\<And>n. n < t \<Longrightarrow> lookup \<tau> n = 0"
+  assumes "b_conc_exec t \<sigma> \<gamma> \<theta> nand3 \<tau> = \<tau>'"
+  assumes "s \<noteq> C"
+  shows "\<And>i. signal_of \<tau> s i = signal_of \<tau>' s i"
+  using b_conc_exec_does_not_modify_signals[OF assms(1-2)] assms(3)
+  unfolding nand3_def by auto
+
+lemma maxtime_maxtime_bigstep:
+  assumes "maxtime, maxtime, \<sigma>, \<gamma>, \<theta> \<turnstile> <nand3, \<tau>> \<leadsto> beh"
+  assumes "\<And>n. n < maxtime \<Longrightarrow> lookup \<tau> n = 0"
+  assumes "\<And>n. maxtime \<le> n \<Longrightarrow> lookup \<theta> n = 0"
+  shows "beh = Poly_Mapping.update maxtime (Some o \<sigma>) \<theta>"
+proof (cases "quiet \<tau> \<gamma>")
+  case True
+  then show ?thesis
+    using case_quiesce[OF _ True assms(1)] by auto
+next
+  case False
+  then obtain \<tau>' where cyc: "maxtime, \<sigma>, \<gamma>, \<theta> \<turnstile> <nand3, rem_curr_trans maxtime \<tau>> \<longrightarrow>\<^sub>c \<tau>'" and
+    big: "maxtime, next_time maxtime \<tau>', next_state maxtime \<tau>' \<sigma>, next_event maxtime \<tau>' \<sigma>,
+                        add_to_beh \<sigma> \<theta> maxtime (next_time maxtime \<tau>') \<turnstile> <nand3, \<tau>'> \<leadsto> beh"
+    using case_bau2[OF _ False assms(1)] by auto
+  have 0: "\<And>n. n < maxtime \<Longrightarrow> lookup \<tau>' n = 0"
+    using b_conc_exec_rem_curr_trans_preserve_trans_removal[OF assms(2)] cyc by auto
+  have "maxtime \<le> next_time maxtime \<tau>'"
+    using next_time_at_least[OF 0, of "maxtime"] by auto
+
+  define \<sigma>2 where "\<sigma>2 = next_state maxtime \<tau>' \<sigma>"
+  define \<gamma>2 where "\<gamma>2 = next_event maxtime \<tau>' \<sigma>"
+  hence big2: "maxtime, next_time maxtime \<tau>', \<sigma>2, \<gamma>2, add_to_beh \<sigma> \<theta> maxtime (next_time maxtime \<tau>')
+                                                                              \<turnstile> <nand3, \<tau>'> \<leadsto> beh"
+    using big unfolding  \<sigma>2_def \<gamma>2_def by auto
+  have "\<tau>' = 0 \<or> \<tau>' \<noteq> 0"
+    by auto
+  moreover
+  { assume "\<tau>' = 0"
+    hence ntime: "next_time maxtime \<tau>' = maxtime"
+      by auto
+    hence ntheta: "add_to_beh \<sigma> \<theta> maxtime (next_time maxtime \<tau>') = \<theta>"
+      by auto
+    have "\<sigma>2 = \<sigma>"
+      unfolding `\<tau>' = 0` \<sigma>2_def next_state_def by auto
+    hence "\<gamma>2 = {}"
+      unfolding `\<tau>' = 0` \<gamma>2_def next_event_def by (simp add: domIff zero_map)
+    hence "quiet \<tau>' \<gamma>2"
+      using `\<tau>' = 0` `\<gamma>2 = {}` unfolding quiet_def by auto
+    have "beh = Poly_Mapping.update maxtime (Some \<circ> \<sigma>) \<theta>"
+      using case_quiesce[OF _ `quiet \<tau>' \<gamma>2` big2] `\<sigma>2 = \<sigma>`
+      unfolding ntime ntheta by auto }
+  moreover
+  { assume "\<tau>' \<noteq> 0"
+    have "disjnt \<gamma> {A, B} \<or> \<not> disjnt \<gamma> {A, B}"
+      by auto
+    moreover
+    { assume "disjnt \<gamma> {A, B}"
+      hence "\<tau>' = rem_curr_trans maxtime \<tau>"
+        using cyc unfolding nand3_def by auto
+      hence "lookup \<tau>' maxtime = 0"
+        unfolding rem_curr_trans_def by (simp add: lookup_update)
+      have max_less: "maxtime < next_time maxtime \<tau>'"
+      proof (rule ccontr)
+        assume "\<not> maxtime < next_time maxtime \<tau>'" hence "maxtime = next_time maxtime \<tau>'"
+          using `maxtime \<le> next_time maxtime \<tau>'` by auto
+        hence least: "(LEAST n. dom (get_trans \<tau>' n) \<noteq> {}) = maxtime"
+          using `\<tau>' \<noteq> 0` unfolding next_time_def  by presburger
+        have "\<exists>n. lookup \<tau>' n \<noteq> 0"
+          using `\<tau>' \<noteq> 0` using aux by blast
+        hence 0: "\<exists>n. dom (lookup \<tau>' n) \<noteq> {}"
+        proof -
+          { assume "dom (0::sig \<Rightarrow> bool option) \<noteq> {}"
+            then have ?thesis
+              by (metis \<open>get_trans \<tau>' maxtime = 0\<close>) }
+          then show ?thesis
+            using \<open>\<exists>n. get_trans \<tau>' n \<noteq> 0\<close> by force
+        qed
+        have "dom (lookup \<tau>' maxtime) \<noteq> {}"
+          using LeastI_ex[OF 0] unfolding least by auto
+        with `lookup \<tau>' maxtime = 0` show "False"
+          by (metis dom_eq_empty_conv zero_map)
+      qed }
+
+    moreover
+    { assume "\<not> disjnt \<gamma> {A, B}"
+      hence \<tau>'_def: "\<tau>' = trans_post C (\<not> (\<sigma> A \<and> \<sigma> B)) (rem_curr_trans maxtime \<tau>) (maxtime + 1)"
+        using cyc unfolding nand3_def by auto
+      hence "\<tau>' \<noteq> 0"
+        unfolding rem_curr_trans_def apply transfer' unfolding trans_post_raw_def
+        by (metis map_upd_nonempty zero_map)
+      hence "next_time maxtime \<tau>' = maxtime + 1"
+      proof -
+        assume "\<tau>' \<noteq> 0"
+        hence "next_time maxtime \<tau>' =  (LEAST n. dom (get_trans \<tau>' n) \<noteq> {})"
+          unfolding next_time_def by auto
+        also have "... = maxtime + 1"
+        proof (rule Least_equality)
+          show " dom (get_trans \<tau>' (maxtime + 1)) \<noteq> {}"
+            unfolding \<tau>'_def rem_curr_trans_def apply transfer' unfolding trans_post_raw_def
+            by auto
+        next
+          { fix y
+            assume "y < maxtime + 1"
+            hence "dom (get_trans \<tau>' y) = {}"
+              unfolding \<tau>'_def rem_curr_trans_def using assms(2) apply transfer' unfolding trans_post_raw_def
+              by (auto simp add: zero_map) }
+          thus "\<And>y. dom (get_trans \<tau>' y) \<noteq> {} \<Longrightarrow> maxtime + 1 \<le> y "
+            by auto
+        qed
+        finally show "next_time maxtime \<tau>' = maxtime + 1"
+          by auto
+      qed
+      hence max_less: "maxtime < next_time maxtime \<tau>'"
+        by auto }
+    ultimately have max_less: "maxtime < next_time maxtime \<tau>'"
+      by auto
+
+    hence new_beh: "add_to_beh \<sigma> \<theta> maxtime (next_time maxtime \<tau>') =  Poly_Mapping.update maxtime (Some o \<sigma>) \<theta>"
+      unfolding add_to_beh_def by auto
+    have "beh =
+      override_lookups_on_open_left (Poly_Mapping.update maxtime (Some \<circ> \<sigma>) \<theta>) 0 maxtime
+                                                                           (next_time maxtime \<tau>')"
+      using max_less case_timesup[OF _ big2] unfolding new_beh by auto
+    also have "... = Poly_Mapping.update maxtime (Some \<circ> \<sigma>) \<theta>"
+      using assms(3) apply transfer' unfolding override_on_def by auto
+    finally have "beh = Poly_Mapping.update maxtime (Some \<circ> \<sigma>) \<theta>"
+      by auto }
+  ultimately show "beh = Poly_Mapping.update maxtime (Some \<circ> \<sigma>) \<theta>"
+    by auto
+qed
+
+lemma t_strictly_increasing:
+  assumes "t, \<sigma>, \<gamma>, \<theta> \<turnstile> <nand3, rem_curr_trans t \<tau>> \<longrightarrow>\<^sub>c \<tau>'"
+  assumes "\<And>n. n < t \<Longrightarrow> lookup \<tau> n = 0"
+  assumes "\<tau>' \<noteq> 0"
+  shows "t < next_time t \<tau>'"
+proof (cases "A \<in> \<gamma> \<or> B \<in> \<gamma>")
+  case True
+  hence \<tau>'_def: "\<tau>' = trans_post C (\<not> (\<sigma> A \<and> \<sigma> B)) (rem_curr_trans t \<tau>) (t + 1)"
+    using assms unfolding nand3_def by auto
+  have "(LEAST n. dom (lookup \<tau>' n) \<noteq> {}) = t + 1"
+  proof (rule Least_equality)
+    show " dom (get_trans \<tau>' (t + 1)) \<noteq> {}"
+      unfolding \<tau>'_def rem_curr_trans_def apply transfer' unfolding trans_post_raw_def by auto
+  next
+    { fix y
+      assume "\<not> t + 1 \<le> y"
+      hence "y < t + 1" by auto
+      hence "lookup \<tau>' y = 0"
+        using assms(2) unfolding \<tau>'_def rem_curr_trans_def apply transfer' unfolding trans_post_raw_def
+        by auto
+      hence "dom (lookup \<tau>' y) = {}"
+        apply transfer' unfolding zero_map by auto }
+    thus "\<And>y. dom (get_trans \<tau>' y) \<noteq> {} \<Longrightarrow> t + 1 \<le> y"
+      by auto
+  qed
+  hence "next_time t \<tau>' = t + 1"
+    using assms(3) unfolding next_time_def by auto
+  thus ?thesis by auto
+next
+  case False
+  hence \<tau>'_def: "\<tau>' = rem_curr_trans t \<tau>"
+    using assms unfolding nand3_def by auto
+  have "lookup \<tau>' t = 0"
+    unfolding \<tau>'_def rem_curr_trans_def by transfer' auto
+  have "next_time t \<tau>' = (LEAST n. dom (lookup \<tau>' n) \<noteq> {})"
+    using assms(3) unfolding next_time_def by auto
+  also have " (LEAST n. dom (lookup \<tau>' n) \<noteq> {}) \<noteq> t"
+  proof (rule ccontr)
+    have asm: "\<exists>x. dom (get_trans \<tau>' x) \<noteq> {}"
+      using `\<tau>' \<noteq> 0` by (metis \<open>get_trans \<tau>' t = 0\<close> aux empty_iff map_add_subsumed1 map_add_subsumed2
+       map_le_def)
+    assume "\<not> (LEAST n. dom (get_trans \<tau>' n) \<noteq> {}) \<noteq> t"
+    hence "dom (lookup \<tau>' t) \<noteq> {}"
+      using LeastI_ex[where P="\<lambda>x. dom (lookup \<tau>' x) \<noteq> {}"] asm by auto
+    hence "lookup \<tau>' t \<noteq> 0"
+      by (metis dom_eq_empty_conv zero_map)
+    with `lookup \<tau>' t = 0` show "False" by auto
+  qed
+  finally have "next_time t \<tau>' \<noteq> t"
+    by auto
+  have *: "\<And>n. n < t \<Longrightarrow> get_trans \<tau>' n = 0"
+    using b_conc_exec_rem_curr_trans_preserve_trans_removal[OF assms(2)] assms(1) by auto
+  have "t \<le> next_time t \<tau>'"
+    using next_time_at_least[OF *, of "t"] by auto
+  with `next_time t \<tau>' \<noteq> t` show ?thesis by auto
+qed
+
+lemma beh_res2:
+  assumes "maxtime, t, \<sigma>, \<gamma>, \<theta> \<turnstile> <cs, \<tau>> \<leadsto> beh"
+  assumes "\<And>n. n < t \<Longrightarrow> lookup \<tau> n = 0"
+  assumes "t \<le> maxtime" and "cs = nand3"
+  assumes "\<And>s. s \<in> dom (lookup \<tau> t) \<Longrightarrow> \<sigma> s = the (lookup \<tau> t s)"
+  assumes "\<And>n. t \<le> n \<Longrightarrow> lookup \<theta> n = 0"
+  shows "\<And>n. n \<le> t \<Longrightarrow> lookup (Poly_Mapping.update t (Some o \<sigma>) \<theta>) n = lookup beh n"
+  using assms
+proof (induction rule:b_simulate_fin.induct)
+  case (1 t maxtime \<tau> \<gamma> \<sigma> \<theta> cs \<tau>' res)
+  have *: "\<And>n. n < t \<Longrightarrow> get_trans \<tau>' n = 0"
+    using b_conc_exec_rem_curr_trans_preserve_trans_removal[OF 1(7)] 1(3) by auto
+  have "t \<le> next_time t \<tau>'"
+    using next_time_at_least[OF *, of "t"] by auto
+  have "\<tau>' = 0 \<or> \<tau>' \<noteq> 0" by auto
+  moreover
+  { assume "\<tau>' = 0"
+    hence "next_time t \<tau>' = t"
+      unfolding next_time_def by auto
+    moreover have " next_state t \<tau>' \<sigma> = \<sigma>"
+      unfolding next_state_def Let_def `next_time t \<tau>' = t` `\<tau>' = 0` override_on_def
+      apply transfer' unfolding zero_map by auto
+    moreover hence "next_event t \<tau>' \<sigma> = {}"
+      unfolding next_event_def next_state_def Let_def `next_time t \<tau>' = t` `\<tau>' = 0`
+      by (auto simp add: zero_map)
+    moreover hence "add_to_beh \<sigma> \<theta> t (next_time t \<tau>') = \<theta>"
+      unfolding `next_time t \<tau>' = t` by auto
+    ultimately have " maxtime, t, \<sigma>, {}, \<theta> \<turnstile> <cs, \<tau>'> \<leadsto> res"
+      using ` maxtime, next_time t \<tau>' , next_state t \<tau>' \<sigma> , next_event t \<tau>' \<sigma> , add_to_beh \<sigma> \<theta> t (next_time t \<tau>') \<turnstile> <cs , \<tau>'> \<leadsto> res`
+      by auto
+    hence "res = Poly_Mapping.update t (Some \<circ> \<sigma>) \<theta>"
+      using case_quiesce[OF `t \<le> maxtime`] unfolding `\<tau>' = 0` quiet_def
+      by (simp add: \<open>\<And>res cs \<theta> \<tau> \<sigma> \<gamma>. \<lbrakk>quiet \<tau> \<gamma>; maxtime, t , \<sigma> , \<gamma> , \<theta> \<turnstile> <cs , \<tau>> \<leadsto> res\<rbrakk>
+                                            \<Longrightarrow> res = Poly_Mapping.update t (Some \<circ> \<sigma>) \<theta>\<close> quiet_def)
+    hence ?case
+      by transfer' auto }
+  moreover
+  { assume "\<tau>' \<noteq> 0"
+    hence "t < next_time t \<tau>'"
+      using t_strictly_increasing[OF _ 1(7) `\<tau>' \<noteq> 0`] 1(3) unfolding `cs = nand3` by auto
+    hence ind1: "n \<le> next_time t \<tau>'"
+      using `n \<le> t` by auto
+    have ind2: "(\<And>n. n < next_time t \<tau>' \<Longrightarrow> get_trans \<tau>' n = 0) "
+      by (simp add: next_time_at_least2)
+    have h1: "\<And>s. s \<in> dom (get_trans \<tau>' (next_time t \<tau>')) \<Longrightarrow>
+                                          next_state t \<tau>' \<sigma> s = the (get_trans \<tau>' (next_time t \<tau>') s)"
+      unfolding next_state_def Let_def by auto
+    have "next_time t \<tau>' \<le> maxtime \<or> maxtime < next_time t \<tau>'"
+      by auto
+    moreover
+    { assume ind3: "next_time t \<tau>' \<le> maxtime"
+      have h2: "\<And>n. next_time t \<tau>' \<le> n \<Longrightarrow> get_trans (add_to_beh \<sigma> \<theta> t (next_time t \<tau>')) n = 0"
+        unfolding add_to_beh_def
+        by (metis (mono_tags) "1.prems"(6) \<open>t < next_time t \<tau>'\<close> \<open>t \<le> next_time t \<tau>'\<close> leD lookup_update order_trans)
+      have "get_trans (Poly_Mapping.update (next_time t \<tau>') (Some \<circ> next_state t \<tau>' \<sigma>) (add_to_beh \<sigma> \<theta> t (next_time t \<tau>'))) n = get_trans res n"
+        using 1(5)[OF ind1 ind2 ind3 `cs = nand3` h1 h2]  by blast
+      hence ?case
+        using `n \<le> t` `t < next_time t \<tau>'` unfolding add_to_beh_def
+      proof -
+        assume a1: "get_trans (Poly_Mapping.update (next_time t \<tau>') (Some \<circ> next_state t \<tau>' \<sigma>) (if t < next_time t \<tau>' then Poly_Mapping.update t (Some \<circ> \<sigma>) \<theta> else \<theta>)) n = get_trans res n"
+        have "next_time t \<tau>' \<noteq> n"
+          using \<open>n \<le> t\<close> \<open>t < next_time t \<tau>'\<close> leD by blast
+        then have "get_trans (Poly_Mapping.update (next_time t \<tau>') (Some \<circ> next_state t \<tau>' \<sigma>) (if t < next_time t \<tau>' then Poly_Mapping.update t (Some \<circ> \<sigma>) \<theta> else \<theta>)) n = get_trans (Poly_Mapping.update t (Some \<circ> \<sigma>) \<theta>) n"
+          by (simp add: \<open>t < next_time t \<tau>'\<close> lookup_update)
+        then show ?thesis
+          using a1 by presburger
+      qed }
+    moreover
+    { assume "maxtime < next_time t \<tau>'"
+      have "t < next_time t \<tau>'"
+        using `t \<le> maxtime` `maxtime < next_time t \<tau>'` by auto
+      have ?case
+        using borderline_big_step[OF 1(4) 1(3) `t \<le> maxtime` `maxtime < next_time t \<tau>'` 1(11) _ ind1]
+        `t < next_time t \<tau>'` unfolding add_to_beh_def  using nat_less_le by presburger }
+    ultimately have ?case by auto }
+  ultimately show ?case by auto
+next
+  case (2 t maxtime \<tau> \<gamma> \<sigma> \<theta> res cs)
+  show ?case
+    using 2(3) by transfer' auto
+next
+  case (3 t maxtime \<theta> res \<sigma> \<gamma> cs \<tau>)
+  then show ?case by auto
+qed
+
+theorem nand3_correctness_ind:
+  assumes "maxtime, t, \<sigma>, \<gamma>, beh \<turnstile> <cs, ctrans> \<leadsto> res"
+  assumes "cs = nand3" and "maxtime = Suc i"
+  assumes "\<And>n. n < t \<Longrightarrow> lookup ctrans n = 0"
+  assumes "\<And>s. s \<in> dom (lookup ctrans t) \<Longrightarrow> \<sigma> s = the (lookup ctrans t s)"
+  assumes "\<And>n. t \<le> n \<Longrightarrow> lookup beh n = 0"
+  assumes "t \<le> i" and "A \<notin> \<gamma> \<and> B \<notin> \<gamma> \<Longrightarrow> \<sigma> C \<longleftrightarrow> \<not> (\<sigma> A \<and> \<sigma> B)"
+  assumes "\<And>n. t < n \<Longrightarrow> lookup (to_transaction2 ctrans C) n = 0"
+  shows "signal_of2 def res C (Suc i) \<longleftrightarrow> \<not> (signal_of2 (\<sigma> A) ctrans A i \<and> signal_of2 (\<sigma> B) ctrans B i)"
+  using assms
+proof (induction rule:b_simulate_fin.induct)
+  case (1 t maxtime \<tau> \<gamma> \<sigma> \<theta> cs \<tau>' res)
+  have "t \<le> Suc i"
+    using `t \<le> i` by auto
+  have *: "\<And>n. n < t \<Longrightarrow> get_trans \<tau>' n = 0"
+    using "1.hyps"(3) "1.prems"(3) b_conc_exec_rem_curr_trans_preserve_trans_removal by blast
+  hence **: "\<And>n. dom (get_trans \<tau>' n) \<noteq> {} \<Longrightarrow> t \<le> n"
+    using zero_map by force
+  hence "t \<le> next_time t \<tau>'"
+    using next_time_at_least[OF *] by auto
+  have h0: "\<And>n. n < next_time t \<tau>' \<Longrightarrow> get_trans \<tau>' n = 0"
+    using b_conc_exec_rem_curr_trans_preserve_trans_removal[OF `\<And>n. n < t \<Longrightarrow> get_trans \<tau> n = 0`]
+    `t , \<sigma> , \<gamma> , \<theta> \<turnstile> <cs , rem_curr_trans t \<tau>> \<longrightarrow>\<^sub>c \<tau>'`  by (simp add: next_time_at_least2)
+
+  have h1: "\<And>s. s \<in> dom (get_trans \<tau>' (next_time t \<tau>')) \<Longrightarrow>
+                                        next_state t \<tau>' \<sigma> s = the (get_trans \<tau>' (next_time t \<tau>') s)"
+    unfolding next_state_def Let_def by auto
+  have h2: "\<And>n. next_time t \<tau>' \<le> n \<Longrightarrow> get_trans (add_to_beh \<sigma> \<theta> t (next_time t \<tau>')) n = 0"
+    unfolding add_to_beh_def
+  proof -
+    fix n :: nat
+    assume a1: "next_time t \<tau>' \<le> n"
+    then have f2: "t \<le> n"
+      by (meson \<open>t \<le> next_time t \<tau>'\<close> order_trans)
+    { assume "n \<noteq> t"
+      then have "get_trans (if t < next_time t \<tau>' then Poly_Mapping.update t (Some \<circ> \<sigma>) \<theta> else \<theta>) n = 0 \<or> next_time t \<tau>' \<le> t"
+        using f2 by (simp add: "1.prems"(5) lookup_update) }
+    then show "get_trans (if t < next_time t \<tau>' then Poly_Mapping.update t (Some \<circ> \<sigma>) \<theta> else \<theta>) n = 0"
+      using a1 "1.prems"(5) \<open>t \<le> next_time t \<tau>'\<close> by fastforce
+  qed
+  { assume asm: "A \<notin> next_event t \<tau>' \<sigma> \<and> B \<notin> next_event t \<tau>' \<sigma> "
+    have sigA: "next_state t \<tau>' \<sigma> A = \<sigma> A" and sigB: "next_state t \<tau>' \<sigma> B = \<sigma> B"
+      using next_state_fixed_point asm by metis+
+    hence "next_event t \<tau>' \<sigma> = {C} \<or> next_event t \<tau>' \<sigma> = {}"
+    proof -
+      have "\<And>S Sa. B \<in> S \<or> S \<subseteq> insert C Sa \<or> A \<in> S"
+        by (metis (full_types) insertI1 sig.exhaust subset_eq)
+      then show ?thesis
+        by (meson \<open>A \<notin> next_event t \<tau>' \<sigma> \<and> B \<notin> next_event t \<tau>' \<sigma>\<close> subset_singletonD)
+    qed
+    moreover
+    { assume "next_event t \<tau>' \<sigma> = {}"
+      hence "C \<notin> next_event t \<tau>' \<sigma>"
+        by auto
+      hence sigC: "next_state t \<tau>' \<sigma> C = \<sigma> C" using next_state_fixed_point[OF `C \<notin> next_event t \<tau>' \<sigma>`]
+        by auto
+      have " A \<notin> \<gamma> \<and> B \<notin> \<gamma>  \<or> \<not> ( A \<notin> \<gamma> \<and> B \<notin> \<gamma> )" by auto
+      moreover
+      { assume " A \<notin> \<gamma> \<and> B \<notin> \<gamma> "
+        hence " \<sigma> C = (\<not> (\<sigma> A \<and> \<sigma> B))"
+          using `A \<notin> \<gamma> \<and> B \<notin> \<gamma> \<Longrightarrow>  \<sigma> C = (\<not> (\<sigma> A \<and> \<sigma> B))` by auto
+        hence " next_state t \<tau>' \<sigma> C = (\<not> (next_state t \<tau>' \<sigma> A \<and> next_state t \<tau>' \<sigma> B))"
+          using sigA sigB sigC by auto }
+      moreover
+      { assume "\<not> ( A \<notin> \<gamma> \<and> B \<notin> \<gamma> )"
+        hence \<tau>'_def: "\<tau>' = trans_post C (\<not> (\<sigma> A \<and> \<sigma> B)) (rem_curr_trans t \<tau>) (t + 1)"
+          using `t , \<sigma> , \<gamma> , \<theta> \<turnstile> <cs , rem_curr_trans t \<tau>> \<longrightarrow>\<^sub>c \<tau>'` unfolding `cs = nand3`
+          nand3_def by auto
+        hence "\<tau>' \<noteq> 0"
+          unfolding rem_curr_trans_def apply transfer' unfolding trans_post_raw_def
+          by (metis map_upd_nonempty zero_map)
+        hence "next_time t \<tau>' = (LEAST n. dom (get_trans \<tau>' n) \<noteq> {})"
+          unfolding next_time_def by auto
+        also have "... = t + 1"
+        proof (rule Least_equality)
+          show "dom (get_trans \<tau>' (t + 1)) \<noteq> {}"
+            unfolding \<tau>'_def rem_curr_trans_def apply transfer' unfolding trans_post_raw_def by auto
+        next
+          have "lookup \<tau>' t = 0"
+            unfolding \<tau>'_def rem_curr_trans_def apply transfer' unfolding trans_post_raw_def
+            by auto
+          thus "\<And>y. dom (get_trans \<tau>' y) \<noteq> {} \<Longrightarrow> t + 1 \<le> y"
+            using **
+            by (metis Suc_eq_plus1 Suc_le_eq dom_eq_empty_conv nat_less_le zero_map)
+        qed
+        finally have "next_time t \<tau>' = t + 1"
+          by auto
+        moreover have "lookup \<tau>' (t + 1) C = Some (\<not> (\<sigma> A \<and> \<sigma> B))"
+          unfolding \<tau>'_def rem_curr_trans_def apply transfer' unfolding trans_post_raw_def by auto
+        ultimately have "next_state t \<tau>' \<sigma> C \<longleftrightarrow> \<not> (\<sigma> A \<and> \<sigma> B)"
+          unfolding next_state_def Let_def  by (simp add: domIff)
+        hence " next_state t \<tau>' \<sigma> C = (\<not> (next_state t \<tau>' \<sigma> A \<and> next_state t \<tau>' \<sigma> B))"
+          using sigA sigB sigC by auto }
+      ultimately have " next_state t \<tau>' \<sigma> C = (\<not> (next_state t \<tau>' \<sigma> A \<and> next_state t \<tau>' \<sigma> B))"
+        by auto }
+    moreover
+    { assume "next_event t \<tau>' \<sigma> = {C}"
+      hence "C \<in> dom (lookup \<tau>' (next_time t \<tau>'))"
+        unfolding next_event_def Let_def by transfer' auto
+      have " A \<notin> \<gamma> \<and> B \<notin> \<gamma>  \<or> \<not> ( A \<notin> \<gamma> \<and> B \<notin> \<gamma> )" by auto
+      moreover
+      { assume "A \<notin> \<gamma> \<and> B \<notin> \<gamma>"
+        hence "\<tau>' = rem_curr_trans t \<tau>"
+          using ` t , \<sigma> , \<gamma> , \<theta> \<turnstile> <cs , rem_curr_trans t \<tau>> \<longrightarrow>\<^sub>c \<tau>'` unfolding `cs = nand3`
+          nand3_def by auto
+        with `\<And>n. t < n \<Longrightarrow> lookup (to_transaction2 \<tau> C) n = 0` and `t \<le> next_time t \<tau>'`
+        have "C \<notin> dom (lookup \<tau>' (next_time t \<tau>'))"
+          unfolding rem_curr_trans_def next_time_def apply transfer' unfolding to_trans_raw2_def
+          by (metis (no_types, lifting) antisym_conv2 domIff fun_upd_apply zero_fun_def zero_map)
+        with `C \<in> dom (lookup \<tau>' (next_time t \<tau>'))` have "False" by auto
+        hence "next_state t \<tau>' \<sigma> C = (\<not> (next_state t \<tau>' \<sigma> A \<and> next_state t \<tau>' \<sigma> B))"
+          by auto }
+      moreover
+      { assume "\<not> ( A \<notin> \<gamma> \<and> B \<notin> \<gamma> )"
+        hence \<tau>'_def: "\<tau>' = trans_post C (\<not> (\<sigma> A \<and> \<sigma> B)) (rem_curr_trans t \<tau>) (t + 1)"
+          using `t , \<sigma> , \<gamma> , \<theta> \<turnstile> <cs , rem_curr_trans t \<tau>> \<longrightarrow>\<^sub>c \<tau>'` unfolding `cs = nand3`
+          nand3_def by auto
+        hence "\<tau>' \<noteq> 0"
+          unfolding rem_curr_trans_def apply transfer' unfolding trans_post_raw_def
+          by (metis map_upd_nonempty zero_map)
+        hence "next_time t \<tau>' = (LEAST n. dom (get_trans \<tau>' n) \<noteq> {})"
+          unfolding next_time_def by auto
+        also have "... = t + 1"
+        proof (rule Least_equality)
+          show "dom (get_trans \<tau>' (t + 1)) \<noteq> {}"
+            unfolding \<tau>'_def rem_curr_trans_def apply transfer' unfolding trans_post_raw_def by auto
+        next
+          have "lookup \<tau>' t = 0"
+            unfolding \<tau>'_def rem_curr_trans_def apply transfer' unfolding trans_post_raw_def
+            by auto
+          thus "\<And>y. dom (get_trans \<tau>' y) \<noteq> {} \<Longrightarrow> t + 1 \<le> y"
+            using **
+            by (metis Suc_eq_plus1 Suc_le_eq dom_eq_empty_conv nat_less_le zero_map)
+        qed
+        finally have "next_time t \<tau>' = t + 1"
+          by auto
+        moreover have "lookup \<tau>' (t + 1) C = Some (\<not> (\<sigma> A \<and> \<sigma> B))"
+          unfolding \<tau>'_def rem_curr_trans_def apply transfer' unfolding trans_post_raw_def by auto
+        ultimately have "next_state t \<tau>' \<sigma> C \<longleftrightarrow> \<not> (\<sigma> A \<and> \<sigma> B)"
+          unfolding next_state_def Let_def  by (simp add: domIff)
+        hence " next_state t \<tau>' \<sigma> C = (\<not> (next_state t \<tau>' \<sigma> A \<and> next_state t \<tau>' \<sigma> B))"
+          using sigA sigB by auto }
+      ultimately have " next_state t \<tau>' \<sigma> C = (\<not> (next_state t \<tau>' \<sigma> A \<and> next_state t \<tau>' \<sigma> B))"
+        by auto }
+    ultimately have "next_state t \<tau>' \<sigma> C = (\<not> (next_state t \<tau>' \<sigma> A \<and> next_state t \<tau>' \<sigma> B))"
+      by auto }
+  note h3 = this
+
+  have h4: "\<And>n. next_time t \<tau>' < n \<Longrightarrow> lookup (to_transaction2 \<tau>' C) n = 0"
+  proof -
+    fix n
+    assume "next_time t \<tau>' < n"
+    have "A \<in> \<gamma> \<or> B \<in> \<gamma> \<or> (A \<notin> \<gamma> \<and> B \<notin> \<gamma>)"
+      by auto
+    moreover
+    { assume "A \<in> \<gamma> \<or> B \<in> \<gamma>"
+      hence \<tau>'_def: "\<tau>' = trans_post C (\<not> (\<sigma> A \<and> \<sigma> B)) (rem_curr_trans t \<tau>) (t + 1)"
+        using `t , \<sigma> , \<gamma> , \<theta> \<turnstile> <cs , rem_curr_trans t \<tau>> \<longrightarrow>\<^sub>c \<tau>'` unfolding `cs = nand3`
+        nand3_def by auto
+      hence "\<tau>' \<noteq> 0"
+        unfolding rem_curr_trans_def apply transfer' unfolding trans_post_raw_def
+        by (metis map_upd_nonempty zero_map)
+      hence "next_time t \<tau>' = (LEAST n. dom (get_trans \<tau>' n) \<noteq> {})"
+        unfolding next_time_def by auto
+      also have "... = t + 1"
+      proof (rule Least_equality)
+        show "dom (get_trans \<tau>' (t + 1)) \<noteq> {}"
+          unfolding \<tau>'_def rem_curr_trans_def apply transfer' unfolding trans_post_raw_def by auto
+      next
+        have "lookup \<tau>' t = 0"
+          unfolding \<tau>'_def rem_curr_trans_def apply transfer' unfolding trans_post_raw_def
+          by auto
+        thus "\<And>y. dom (get_trans \<tau>' y) \<noteq> {} \<Longrightarrow> t + 1 \<le> y"
+          using **
+          by (metis Suc_eq_plus1 Suc_le_eq dom_eq_empty_conv nat_less_le zero_map)
+      qed
+      finally have "next_time t \<tau>' = t + 1"
+        by auto
+      hence "lookup (to_transaction2 \<tau>' C) n = 0"
+        using `next_time t \<tau>' < n` unfolding \<tau>'_def rem_curr_trans_def next_time_def apply transfer'
+        unfolding trans_post_raw_def to_trans_raw2_def
+        by (simp add: zero_option_def) }
+    moreover
+    { assume "A \<notin> \<gamma> \<and> B \<notin> \<gamma>"
+      hence \<tau>'_def: "\<tau>' = rem_curr_trans t \<tau>"
+        using `t , \<sigma> , \<gamma> , \<theta> \<turnstile> <cs , rem_curr_trans t \<tau>> \<longrightarrow>\<^sub>c \<tau>'` unfolding `cs = nand3` nand3_def
+        by auto
+      hence "lookup (to_transaction2 \<tau>' C) n = 0"
+        using `t \<le> next_time t \<tau>'` `next_time t \<tau>' < n` `\<And>n. t < n \<Longrightarrow> lookup (to_transaction2 \<tau> C) n = 0`
+        by (metis leD le_less_trans trans_value_same_except_at_removed) }
+    ultimately show "lookup (to_transaction2 \<tau>' C) n = 0"
+      by auto
+  qed
+
+  have h5: "\<And>n. n < t \<Longrightarrow> get_trans (rem_curr_trans t \<tau>) n = 0"
+    using `\<And>n. n < t \<Longrightarrow> get_trans \<tau> n = 0` unfolding rem_curr_trans_def by transfer' auto
+  have IH: " next_time t \<tau>' \<le> i \<Longrightarrow>
+             signal_of2 def res C (Suc i) =
+            (\<not> (signal_of2 (next_state t \<tau>' \<sigma> A) \<tau>' A i \<and> signal_of2 (next_state t \<tau>' \<sigma> B) \<tau>' B i))"
+    using 1(5)[OF `cs = nand3` `maxtime = Suc i` h0 h1 h2 _ h3 h4] by auto
+  have "i < next_time t \<tau>' \<or> next_time t \<tau>' \<le> i"
+    by auto
+  moreover
+  { assume "i < next_time t \<tau>'"
+    have "t \<noteq> next_time t \<tau>'"
+    proof (rule ccontr)
+      assume "\<not> t \<noteq> next_time t \<tau>'" hence "t = next_time t \<tau>'" by auto
+      hence "i < t"  using `i < next_time t \<tau>'` by auto
+      with `t \<le> i` show False by auto
+    qed
+
+    have "A \<notin> \<gamma> \<and> B \<notin> \<gamma> \<or> A \<in> \<gamma> \<or> B \<in> \<gamma>" by auto
+    moreover
+    { assume "A \<notin> \<gamma> \<and> B \<notin> \<gamma>"
+      hence \<tau>'_def: "\<tau>' = rem_curr_trans t \<tau>"
+        using `t , \<sigma> , \<gamma> , \<theta> \<turnstile> <cs , rem_curr_trans t \<tau>> \<longrightarrow>\<^sub>c \<tau>'` unfolding `cs = nand3` nand3_def
+        by auto
+      have "signal_of2 (\<sigma> A) \<tau> A i = \<sigma> A" and "signal_of2 (\<sigma> B) \<tau> B i = \<sigma> B"
+        using signal_of2_init'[OF `t \<le> i`, of "\<tau>" _ "\<sigma>"] `i < next_time t \<tau>'` 1(9) 1(8)
+        unfolding \<tau>'_def by auto
+      note no_trans_c = 1(13)
+      hence "\<And>n. t \<le> n \<Longrightarrow> lookup (to_transaction2 \<tau>' C) n = 0"
+        unfolding \<tau>'_def unfolding rem_curr_trans_def apply transfer' unfolding to_trans_raw2_def
+        by (simp add: zero_fun_def)
+      note next_big_step = 1(4)
+      have "next_time t \<tau>' \<le> maxtime \<or> maxtime < next_time t \<tau>'" by auto
+      moreover
+      { assume "next_time t \<tau>' \<le> maxtime"
+        hence pre: "\<And>n. n < next_time t \<tau>' \<Longrightarrow> get_trans (add_to_beh \<sigma> \<theta> t (next_time t \<tau>')) n = get_trans res n"
+          using   beh_res[OF next_big_step h0] by auto
+        hence "\<And>n. n < next_time t \<tau>' \<Longrightarrow> lookup (Poly_Mapping.update t (Some o \<sigma>) \<theta>) n = lookup res n"
+          using`t \<le> next_time t \<tau>'` `t \<noteq> next_time t \<tau>'` unfolding add_to_beh_def by auto
+        hence *: "\<And>n. n \<le> next_time t \<tau>' \<Longrightarrow>
+            get_trans (Poly_Mapping.update (next_time t \<tau>') (Some \<circ> next_state t \<tau>' \<sigma>) (add_to_beh \<sigma> \<theta> t (next_time t \<tau>'))) n = get_trans res n"
+          using beh_res2[OF next_big_step h0 `next_time t \<tau>' \<le> maxtime` `cs = nand3` h1 h2 ]
+          by auto
+        have "Suc i \<le> next_time t \<tau>'"
+          using `i < next_time t \<tau>'` `next_time t \<tau>' \<le> maxtime` by auto
+        hence "Suc i < next_time t \<tau>' \<or> Suc i = next_time t \<tau>'"
+          by auto
+        moreover
+        { assume "Suc i < next_time t \<tau>'"
+          hence "Suc i < next_time t (rem_curr_trans t \<tau>)"
+            unfolding \<tau>'_def by auto
+          hence "signal_of2 def res C (Suc i) =
+                 signal_of2 def (add_to_beh \<sigma> \<theta> t (next_time t \<tau>')) C (Suc i)"
+            using signal_of2_lookup_same[OF pre]  "1.prems"(2) \<open>next_time t \<tau>' \<le> maxtime\<close> `Suc i < next_time t \<tau>'`
+            by linarith
+          also have "... =  signal_of2 def (Poly_Mapping.update t (Some o \<sigma>) \<theta>) C (Suc i)"
+            unfolding add_to_beh_def using `t \<le> next_time t \<tau>'` `t \<noteq> next_time t \<tau>'` by auto
+          also have "... = \<sigma> C"
+          proof -
+            have "inf_time (to_transaction2 (Poly_Mapping.update t (Some o \<sigma>) \<theta>)) C (Suc i) = Some t"
+              using inf_time_update[OF 1(10)]  using \<open>t \<le> Suc i\<close> by blast
+            thus ?thesis
+              unfolding to_signal2_def comp_def
+              using "1.prems"(2) \<open>Suc i < next_time t \<tau>'\<close> \<open>next_time t \<tau>' \<le> maxtime\<close> leD by blast
+          qed
+          finally have "signal_of2 def res C (Suc i) = \<sigma> C"
+            by auto
+          moreover have "\<sigma> C \<longleftrightarrow> \<not> (\<sigma> A \<and> \<sigma> B)"
+            using 1(12) `A \<notin> \<gamma> \<and> B \<notin> \<gamma>` by auto
+          ultimately have ?case
+            using `signal_of2 (\<sigma> A) \<tau> A i = \<sigma> A` `signal_of2 (\<sigma> B) \<tau> B i = \<sigma> B` by auto }
+        moreover
+        { assume "Suc i = next_time t \<tau>'"
+          hence **: "signal_of2 def res C (Suc i) =
+                 signal_of2 def (Poly_Mapping.update (next_time t \<tau>') (Some \<circ> next_state t \<tau>' \<sigma>) (add_to_beh \<sigma> \<theta> t (next_time t \<tau>'))) C (Suc i)"
+            using signal_of2_lookup_same[OF * `Suc i \<le> next_time t \<tau>'`] by auto
+          define t' where "t' = next_time t \<tau>'"
+          define \<sigma>' where "\<sigma>' = next_state t \<tau>' \<sigma>"
+          define \<theta>' where "\<theta>' = add_to_beh \<sigma> \<theta> t (next_time t \<tau>')"
+          hence "signal_of2 def res C (Suc i) =
+                 signal_of2 def (Poly_Mapping.update t' (Some o \<sigma>') \<theta>') C (Suc i)"
+            unfolding t'_def \<sigma>'_def \<theta>'_def using ** by auto
+          also have "... = \<sigma>' C"
+          proof -
+            have "next_time t \<tau>' \<le> Suc i"
+              using `Suc i = next_time t \<tau>'` by auto
+            hence "inf_time (to_transaction2 (Poly_Mapping.update t' (\<lambda>x. Some (\<sigma>' x)) \<theta>')) C (Suc i) = Some t'"
+              using inf_time_update[OF h2 _ `next_time t \<tau>' \<le> Suc i`, of "\<sigma>'"] unfolding \<theta>'_def t'_def comp_def
+              by blast
+            thus ?thesis
+              unfolding to_signal2_def comp_def
+              by (simp add: lookup_update to_trans_raw2_def to_transaction2.rep_eq)
+          qed
+          finally have "signal_of2 def res C (Suc i) = \<sigma>' C"
+            by auto
+          also have "... = \<sigma> C"
+          proof -
+            have "C \<notin> dom (lookup (rem_curr_trans t \<tau>) (i + 1))"
+              using 1(13) `t \<le> Suc i`
+              unfolding rem_curr_trans_def apply transfer' unfolding to_trans_raw2_def
+              by (auto simp add: zero_map zero_option_def)
+            moreover have *: "(next_time t (rem_curr_trans t \<tau>)) = i + 1"
+              using `Suc i = next_time t \<tau>'` unfolding \<tau>'_def by auto
+            ultimately show ?thesis
+              unfolding \<sigma>'_def next_state_def \<tau>'_def * Let_def by auto
+          qed
+          finally have "signal_of2 def res C (Suc i) = \<sigma> C"
+            by auto
+          moreover have "\<sigma> C \<longleftrightarrow> \<not> (\<sigma> A \<and> \<sigma> B)"
+            using 1(12) `A \<notin> \<gamma> \<and> B \<notin> \<gamma>` by auto
+          ultimately have ?case
+            using `signal_of2 (\<sigma> A) \<tau> A i = \<sigma> A` `signal_of2 (\<sigma> B) \<tau> B i = \<sigma> B` by auto }
+        ultimately have ?case by auto }
+      moreover
+      { assume "maxtime < next_time t \<tau>'"
+        hence pre: "\<And>n. n \<le> next_time t \<tau>' \<Longrightarrow> get_trans (add_to_beh \<sigma> \<theta> t (next_time t \<tau>')) n = get_trans res n"
+          using borderline_big_step[OF next_big_step `t , \<sigma> , \<gamma> , \<theta> \<turnstile> <cs , rem_curr_trans t \<tau>> \<longrightarrow>\<^sub>c \<tau>'` `t \<le> maxtime` `maxtime < next_time t \<tau>'` 1(10)]
+          by auto
+        have "Suc i < next_time t \<tau>'"
+          using `maxtime = Suc i` `maxtime < next_time t \<tau>'` by auto
+        hence "Suc i < next_time t (rem_curr_trans t \<tau>)"
+          unfolding \<tau>'_def by auto
+        hence "signal_of2 def res C (Suc i) =
+               signal_of2 def (add_to_beh \<sigma> \<theta> t (next_time t \<tau>')) C (Suc i)"
+          using signal_of2_lookup_same[OF pre] `Suc i < next_time t \<tau>'` by auto
+        also have "... =  signal_of2 def (Poly_Mapping.update t (Some o \<sigma>) \<theta>) C (Suc i)"
+          unfolding add_to_beh_def using `t \<le> next_time t \<tau>'` `t \<noteq> next_time t \<tau>'` by auto
+        also have "... = \<sigma> C"
+        proof -
+          have "inf_time (to_transaction2 (Poly_Mapping.update t (Some o \<sigma>) \<theta>)) C (Suc i) = Some t"
+            using inf_time_update[OF 1(10)]  using \<open>t \<le> Suc i\<close> by blast
+          thus ?thesis
+            unfolding to_signal2_def comp_def
+            by (simp add: lookup_update to_trans_raw2_def to_transaction2.rep_eq)
+        qed
+        finally have "signal_of2 def res C (Suc i) = \<sigma> C"
+          by auto
+        moreover have "\<sigma> C \<longleftrightarrow> \<not> (\<sigma> A \<and> \<sigma> B)"
+          using 1(12) `A \<notin> \<gamma> \<and> B \<notin> \<gamma>` by auto
+        ultimately have ?case
+          using `signal_of2 (\<sigma> A) \<tau> A i = \<sigma> A` `signal_of2 (\<sigma> B) \<tau> B i = \<sigma> B` by auto }
+      ultimately have ?case by auto }
+    moreover
+    { assume "A \<in> \<gamma> \<or> B \<in> \<gamma>"
+      hence \<tau>'_def: "\<tau>' = trans_post C (\<not> (\<sigma> A \<and> \<sigma> B)) (rem_curr_trans t \<tau>) (t+1)"
+        using `t , \<sigma> , \<gamma> , \<theta> \<turnstile> <cs , rem_curr_trans t \<tau>> \<longrightarrow>\<^sub>c \<tau>'` unfolding `cs = nand3` nand3_def
+        by auto
+      hence "\<tau>' \<noteq> 0"
+        unfolding rem_curr_trans_def apply transfer' unfolding trans_post_raw_def
+        by (metis map_upd_nonempty zero_map)
+      hence "next_time t \<tau>' = (LEAST n. dom (lookup \<tau>' n) \<noteq> {})"
+        unfolding next_time_def by auto
+      also have "... = t + 1"
+      proof (rule Least_equality)
+        show "dom (get_trans \<tau>' (t + 1)) \<noteq> {}"
+          unfolding \<tau>'_def rem_curr_trans_def apply transfer' unfolding trans_post_raw_def by auto
+      next
+        { fix y
+          assume "\<not> t + 1 \<le> y" hence "y < t + 1" by auto
+          hence "dom (get_trans \<tau>' y) = {}"
+            using 1(8) unfolding \<tau>'_def rem_curr_trans_def apply transfer' unfolding trans_post_raw_def
+            by (auto simp add:zero_map) }
+        thus "\<And>y. dom (get_trans \<tau>' y) \<noteq> {} \<Longrightarrow> t + 1 \<le> y"
+          by auto
+      qed
+      finally have "next_time t \<tau>' = t + 1"
+        by auto
+      with `i < next_time t \<tau>'` have "i < t + 1" by auto
+      with `t \<le> i` have "i = t" by auto
+      hence "signal_of2 (\<sigma> A) \<tau> A i = signal_of2 (\<sigma> A) \<tau> A t"
+        by auto
+      also have "... = \<sigma> A"
+      proof -
+      consider "inf_time (to_transaction2 \<tau>) A t = None" |  ta where "inf_time (to_transaction2 \<tau>) A t = Some ta"
+        by blast
+      thus ?thesis
+      proof (cases)
+        case 1
+        then show ?thesis unfolding to_signal2_def comp_def by auto
+      next
+        case 2
+        have "t = ta"
+        proof (rule ccontr)
+          assume "t \<noteq> ta"
+          with 2 have "ta \<le> t" by (auto dest!:inf_time_at_most)
+          with `t \<noteq> ta` have "ta < t" by auto
+          hence "lookup \<tau> ta = 0"
+            using 1(8) by auto
+          have "ta \<in> dom (lookup (to_transaction2 \<tau> A))"
+            using inf_time_someE2[OF 2] by auto
+          hence "lookup (to_transaction2 \<tau> A) ta \<noteq> 0"
+            apply transfer' unfolding to_trans_raw2_def by (metis domIff zero_fun_def zero_map)
+          hence "lookup \<tau> ta \<noteq> 0"
+            apply transfer' unfolding to_trans_raw2_def by (metis zero_fun_def)
+          thus False
+            using `lookup \<tau> ta = 0` by auto
+        qed
+        hence "inf_time (to_transaction2 \<tau>) A t = Some t"
+          using 2 by auto
+        hence "t \<in> dom (lookup (to_transaction2 \<tau> A))"
+          by (auto dest!:inf_time_someE2)
+        hence "A \<in> dom (get_trans \<tau> t)"
+          apply transfer' unfolding to_trans_raw2_def by auto
+        hence "the (lookup (to_transaction2 \<tau> A) t) = \<sigma> A"
+          using 1(9) apply transfer' unfolding to_trans_raw2_def by auto
+        then show ?thesis
+          using `inf_time (to_transaction2 \<tau>) A t = Some t` unfolding to_signal2_def comp_def
+          by auto
+      qed
+      qed
+      finally have sigA: "signal_of2 (\<sigma> A) \<tau> A i = \<sigma> A"
+        by auto
+      have "signal_of2 (\<sigma> B) \<tau> B i = signal_of2 (\<sigma> B) \<tau> B t"
+        using `i = t` by auto
+      also have "... = \<sigma> B"
+      proof -
+      consider "inf_time (to_transaction2 \<tau>) B t = None" |  ta where "inf_time (to_transaction2 \<tau>) B t = Some ta"
+        by blast
+      thus ?thesis
+      proof (cases)
+        case 1
+        then show ?thesis unfolding to_signal2_def comp_def by auto
+      next
+        case 2
+        have "t = ta"
+        proof (rule ccontr)
+          assume "t \<noteq> ta"
+          with 2 have "ta \<le> t" by (auto dest!:inf_time_at_most)
+          with `t \<noteq> ta` have "ta < t" by auto
+          hence "lookup \<tau> ta = 0"
+            using 1(8) by auto
+          have "ta \<in> dom (lookup (to_transaction2 \<tau> B))"
+            using inf_time_someE2[OF 2] by auto
+          hence "lookup (to_transaction2 \<tau> B) ta \<noteq> 0"
+            apply transfer' unfolding to_trans_raw2_def by (metis domIff zero_fun_def zero_map)
+          hence "lookup \<tau> ta \<noteq> 0"
+            apply transfer' unfolding to_trans_raw2_def by (metis zero_fun_def)
+          thus False
+            using `lookup \<tau> ta = 0` by auto
+        qed
+        hence "inf_time (to_transaction2 \<tau>) B t = Some t"
+          using 2 by auto
+        hence "t \<in> dom (lookup (to_transaction2 \<tau> B))"
+          by (auto dest!:inf_time_someE2)
+        hence "B \<in> dom (get_trans \<tau> t)"
+          apply transfer' unfolding to_trans_raw2_def by auto
+        hence "the (lookup (to_transaction2 \<tau> B) t) = \<sigma> B"
+          using 1(9) apply transfer' unfolding to_trans_raw2_def by auto
+        then show ?thesis
+          using `inf_time (to_transaction2 \<tau>) B t = Some t` unfolding to_signal2_def comp_def
+          by auto
+      qed
+      qed
+      finally have sigB: "signal_of2 (\<sigma> B) \<tau> B i = \<sigma> B"
+        by auto
+      note next_big_step = 1(4)
+      have "next_time t \<tau>' \<le> maxtime"
+        using `next_time t \<tau>' = t + 1` `maxtime = Suc i` `i = t` by auto
+      have "\<And>n. n \<le> next_time t \<tau>' \<Longrightarrow>
+            get_trans (Poly_Mapping.update (next_time t \<tau>') (Some \<circ> next_state t \<tau>' \<sigma>) (add_to_beh \<sigma> \<theta> t (next_time t \<tau>'))) n = get_trans res n"
+        using beh_res2[OF next_big_step h0 `next_time t \<tau>' \<le> maxtime` `cs = nand3` h1 h2] by auto
+      hence "lookup res (next_time t \<tau>') = (Some o next_state t \<tau>' \<sigma>)"
+        by (metis lookup_update order_refl)
+      hence "lookup res (Suc i) = (Some o next_state t \<tau>' \<sigma>)"
+        using `next_time t \<tau>' = t + 1` `i = t` by auto
+      hence "signal_of2 def res C (Suc i) = next_state t \<tau>' \<sigma> C"
+        by (auto dest!: lookup_some_signal_of2)
+      also have "... = (let m = get_trans \<tau>' (t + 1) in override_on \<sigma> (the o m) (dom m)) C"
+        using `next_time t \<tau>' = t + 1` unfolding next_state_def by auto
+      also have "... \<longleftrightarrow> \<not> (\<sigma> A \<and> \<sigma> B)"
+        unfolding Let_def \<tau>'_def rem_curr_trans_def apply transfer' unfolding trans_post_raw_def
+        by auto
+      finally have "signal_of2 def res C (Suc i) \<longleftrightarrow> \<not> (\<sigma> A \<and> \<sigma> B)"
+        by auto
+      hence ?case
+        using sigA sigB by auto }
+    ultimately have ?case by auto }
+  moreover
+  { assume "next_time t \<tau>' \<le> i"
+    with IH have IH': "signal_of2 def res C (Suc i) =
+            (\<not> (signal_of2 (next_state t \<tau>' \<sigma> A) \<tau>' A i \<and> signal_of2 (next_state t \<tau>' \<sigma> B) \<tau>' B i))"
+      by auto
+    have Anot: "A \<notin> set (signals_from cs)"
+      unfolding `cs = nand3` nand3_def by auto
+    have "signal_of2 (next_state t \<tau>' \<sigma> A) \<tau>' A i  = signal_of2 (\<sigma> A) (rem_curr_trans t \<tau>) A i"
+      using b_conc_exec_does_not_modify_signals2[OF h5 `t , \<sigma> , \<gamma> , \<theta> \<turnstile> <cs , rem_curr_trans t \<tau>> \<longrightarrow>\<^sub>c \<tau>'` Anot `next_time t \<tau>' \<le> i`]
+      unfolding `cs = nand3` nand3_def by auto
+    also have "... = signal_of2 (\<sigma> A) \<tau> A i"
+    proof -
+      obtain ta where  "inf_time (to_transaction2 \<tau>) A i = None \<or>  inf_time (to_transaction2 \<tau>) A i = Some ta"
+        (is "?none \<or> ?some")
+        using option.exhaust_sel by blast
+      moreover
+      { assume "?none"
+        hence "\<forall>t \<in> dom (lookup (to_transaction2 \<tau> A)). i < t"
+          by (auto dest!:inf_time_noneE)
+        moreover have "dom (lookup (to_transaction2 (rem_curr_trans t \<tau>) A)) \<subseteq> dom (lookup (to_transaction2 \<tau> A))"
+          unfolding rem_curr_trans_def apply transfer' unfolding to_trans_raw2_def
+          by (simp add: Collect_mono dom_def zero_map)
+        ultimately have "\<forall>t \<in> dom (lookup (to_transaction2 (rem_curr_trans t \<tau>) A)). i < t"
+          by (simp add: subset_iff)
+        hence "inf_time (to_transaction2 (rem_curr_trans t \<tau>)) A i = None"
+          by (auto intro!: inf_time_noneI)
+        hence ?thesis using `?none` unfolding to_signal2_def comp_def
+          by auto }
+      moreover
+      { assume "?some"
+        hence "ta \<in> dom (lookup (to_transaction2 \<tau> A))" and *: "\<forall>t \<in> dom (lookup (to_transaction2 \<tau> A)). t \<le> i \<longrightarrow> t \<le> ta"
+          using inf_time_someE2[OF `?some`] inf_time_someE[OF `?some`] by auto
+        have "ta = t \<or> ta \<noteq> t" by auto
+        moreover
+        { assume "ta \<noteq> t"
+          hence "inf_time (to_transaction2 (rem_curr_trans t \<tau>)) A i = Some ta"
+            using `?some` by (simp add: inf_time_rem_curr_trans)
+          moreover have "lookup (to_transaction2 (rem_curr_trans t \<tau>) A) ta = lookup (to_transaction2 \<tau> A) ta"
+            using `ta \<noteq> t` unfolding rem_curr_trans_def apply transfer' unfolding to_trans_raw2_def by auto
+          ultimately have ?thesis using `?some` unfolding to_signal2_def comp_def
+            using `ta \<noteq> t` by auto }
+        moreover
+        { assume "ta = t"
+          hence "A \<in> dom (get_trans \<tau> t)"
+            using `ta \<in> dom (lookup (to_transaction2 \<tau> A))` apply transfer' unfolding to_trans_raw2_def
+            by auto
+          have "\<forall>k \<in> dom (lookup (to_transaction2 \<tau> A)). k \<le> i \<longrightarrow> k \<le> t"
+            using * `ta = t` by auto
+          moreover have "dom (lookup (to_transaction2 (rem_curr_trans t \<tau>) A)) \<subseteq> dom (lookup (to_transaction2 \<tau> A))"
+            unfolding rem_curr_trans_def apply transfer' unfolding to_trans_raw2_def
+            by (simp add: Collect_mono dom_def zero_map)
+          moreover have "\<forall>k \<in> dom (lookup (to_transaction2 (rem_curr_trans t \<tau>) A)). k > t"
+            using 1(8) unfolding rem_curr_trans_def apply transfer' unfolding to_trans_raw2_def
+            by (metis domIff fun_upd_apply nat_neq_iff zero_map)
+          ultimately have "\<forall>k \<in> dom (lookup (to_transaction2 (rem_curr_trans t \<tau>) A)). i < k"
+            by (meson leD le_less_linear subset_iff)
+          hence "inf_time (to_transaction2 (rem_curr_trans t \<tau>)) A i = None"
+            by (auto intro!: inf_time_noneI)
+          hence "signal_of2 (\<sigma> A) (rem_curr_trans t \<tau>) A i = \<sigma> A"
+            unfolding to_signal2_def comp_def by auto
+          also have "... = the (lookup \<tau> t A)"
+            using `\<And>s. s \<in> dom (get_trans \<tau> t) \<Longrightarrow> \<sigma> s = the (get_trans \<tau> t s)` `A \<in> dom (get_trans \<tau> t)`
+            by auto
+          finally have ?thesis
+            using `?some` `ta = t` unfolding to_signal2_def comp_def
+            by (simp add: to_trans_raw2_def to_transaction2.rep_eq) }
+        ultimately have ?thesis by auto }
+      ultimately show ?thesis by auto
+    qed
+    finally have "signal_of2 (next_state t \<tau>' \<sigma> A) \<tau>' A i  = signal_of2 (\<sigma> A) \<tau> A i"
+      by auto
+
+    have Bnot: "B \<notin> set (signals_from cs)"
+      unfolding `cs = nand3` nand3_def by auto
+    have "signal_of2 (next_state t \<tau>' \<sigma> B) \<tau>' B i  = signal_of2 (\<sigma> B) (rem_curr_trans t \<tau>) B i"
+      using b_conc_exec_does_not_modify_signals2[OF h5 `t , \<sigma> , \<gamma> , \<theta> \<turnstile> <cs , rem_curr_trans t \<tau>> \<longrightarrow>\<^sub>c \<tau>'` Bnot `next_time t \<tau>' \<le> i`]
+      unfolding `cs = nand3` nand3_def by auto
+    also have "... = signal_of2 (\<sigma> B) \<tau> B i"
+    proof -
+      obtain ta where  "inf_time (to_transaction2 \<tau>) B i = None \<or>  inf_time (to_transaction2 \<tau>) B i = Some ta"
+        (is "?none \<or> ?some")
+        using option.exhaust_sel by blast
+      moreover
+      { assume "?none"
+        hence "\<forall>t \<in> dom (lookup (to_transaction2 \<tau> B)). i < t"
+          by (auto dest!:inf_time_noneE)
+        moreover have "dom (lookup (to_transaction2 (rem_curr_trans t \<tau>) B)) \<subseteq> dom (lookup (to_transaction2 \<tau> B))"
+          unfolding rem_curr_trans_def apply transfer' unfolding to_trans_raw2_def
+          by (simp add: Collect_mono dom_def zero_map)
+        ultimately have "\<forall>t \<in> dom (lookup (to_transaction2 (rem_curr_trans t \<tau>) B)). i < t"
+          by (simp add: subset_iff)
+        hence "inf_time (to_transaction2 (rem_curr_trans t \<tau>)) B i = None"
+          by (auto intro!: inf_time_noneI)
+        hence ?thesis using `?none` unfolding to_signal2_def comp_def
+          by auto }
+      moreover
+      { assume "?some"
+        hence "ta \<in> dom (lookup (to_transaction2 \<tau> B))" and *: "\<forall>t \<in> dom (lookup (to_transaction2 \<tau> B)). t \<le> i \<longrightarrow> t \<le> ta"
+          using inf_time_someE2[OF `?some`] inf_time_someE[OF `?some`] by auto
+        have "ta = t \<or> ta \<noteq> t" by auto
+        moreover
+        { assume "ta \<noteq> t"
+          hence "inf_time (to_transaction2 (rem_curr_trans t \<tau>)) B i = Some ta"
+            using `?some` by (simp add: inf_time_rem_curr_trans)
+          moreover have "lookup (to_transaction2 (rem_curr_trans t \<tau>) B) ta = lookup (to_transaction2 \<tau> B) ta"
+            using `ta \<noteq> t` unfolding rem_curr_trans_def apply transfer' unfolding to_trans_raw2_def by auto
+          ultimately have ?thesis using `?some` unfolding to_signal2_def comp_def
+            using `ta \<noteq> t` by auto }
+        moreover
+        { assume "ta = t"
+          hence "B \<in> dom (get_trans \<tau> t)"
+            using `ta \<in> dom (lookup (to_transaction2 \<tau> B))` apply transfer' unfolding to_trans_raw2_def
+            by auto
+          have "\<forall>k \<in> dom (lookup (to_transaction2 \<tau> B)). k \<le> i \<longrightarrow> k \<le> t"
+            using * `ta = t` by auto
+          moreover have "dom (lookup (to_transaction2 (rem_curr_trans t \<tau>) B)) \<subseteq> dom (lookup (to_transaction2 \<tau> B))"
+            unfolding rem_curr_trans_def apply transfer' unfolding to_trans_raw2_def
+            by (simp add: Collect_mono dom_def zero_map)
+          moreover have "\<forall>k \<in> dom (lookup (to_transaction2 (rem_curr_trans t \<tau>) B)). k > t"
+            using 1(8) unfolding rem_curr_trans_def apply transfer' unfolding to_trans_raw2_def
+            by (metis domIff fun_upd_apply nat_neq_iff zero_map)
+          ultimately have "\<forall>k \<in> dom (lookup (to_transaction2 (rem_curr_trans t \<tau>) B)). i < k"
+            by (meson leD le_less_linear subset_iff)
+          hence "inf_time (to_transaction2 (rem_curr_trans t \<tau>)) B i = None"
+            by (auto intro!: inf_time_noneI)
+          hence "signal_of2 (\<sigma> B) (rem_curr_trans t \<tau>) B i = \<sigma> B"
+            unfolding to_signal2_def comp_def by auto
+          also have "... = the (lookup \<tau> t B)"
+            using `\<And>s. s \<in> dom (get_trans \<tau> t) \<Longrightarrow> \<sigma> s = the (get_trans \<tau> t s)` `B \<in> dom (get_trans \<tau> t)`
+            by auto
+          finally have ?thesis
+            using `?some` `ta = t` unfolding to_signal2_def comp_def
+            by (simp add: to_trans_raw2_def to_transaction2.rep_eq) }
+        ultimately have ?thesis by auto }
+      ultimately show ?thesis by auto
+    qed
+    finally have "signal_of2 (next_state t \<tau>' \<sigma> B) \<tau>' B i  = signal_of2 (\<sigma> B) \<tau> B i"
+      by auto
+    hence ?case
+      using `signal_of2 (next_state t \<tau>' \<sigma> A) \<tau>' A i  = signal_of2 (\<sigma> A) \<tau> A i` IH'
+      by auto }
+  ultimately show ?case by auto
+next
+  case (2 t maxtime \<tau> \<gamma> \<sigma> \<theta> res cs)
+  have "\<tau> = 0"
+    using `quiet \<tau> \<gamma>` unfolding quiet_def by metis
+  hence *: "signal_of2 (\<sigma> A) \<tau> A i = \<sigma> A" and **: "signal_of2 (\<sigma> B) \<tau> B i = \<sigma> B"
+    unfolding to_signal2_def by auto
+  have "inf_time (to_transaction2 res) C (Suc i) = Some t"
+    using inf_time_update[OF `\<And>n. t \<le> n \<Longrightarrow> get_trans \<theta> n = 0` ` Poly_Mapping.update t (Some \<circ> \<sigma>) \<theta> = res`
+    `t \<le> maxtime`] unfolding  `maxtime = Suc i` by auto
+  hence "signal_of2 def res C (Suc i) = \<sigma> C"
+    using `Poly_Mapping.update t (Some \<circ> \<sigma>) \<theta> = res` unfolding to_signal2_def comp_def
+    unfolding inf_time_def apply transfer' unfolding to_trans_raw2_def by auto
+  moreover have "A \<notin> \<gamma> \<and> B \<notin> \<gamma>"
+    using `quiet \<tau> \<gamma>` unfolding quiet_def  by (metis emptyE)
+  ultimately show ?case
+    using * ** 2(10)[OF `A \<notin> \<gamma> \<and> B \<notin> \<gamma>`]  by auto
+next
+  case (3 t maxtime \<theta> res \<sigma> \<gamma> cs \<tau>)
+  then show ?case by auto
+qed
+
+lemma signal_of2_cong_neq_none_at_0:
+  assumes "lookup (to_transaction2 \<tau> sig) 0 \<noteq> None"
+  shows "signal_of2 def1 \<tau> sig i = signal_of2 def2 \<tau> sig i"
+proof -
+  have "inf_time (to_transaction2 \<tau>) sig i \<noteq> None"
+  proof (rule ccontr)
+    assume "\<not> inf_time (to_transaction2 \<tau>) sig i \<noteq> None"
+    hence "inf_time (to_transaction2 \<tau>) sig i = None"
+      by auto
+    hence "\<forall>k. k \<le> i \<longrightarrow> lookup (to_transaction2 \<tau> sig) k = 0"
+      by (auto dest!: inf_time_noneE2)
+    hence "lookup (to_transaction2 \<tau> sig) 0 = 0"
+      by auto
+    with assms show "False"
+      by (simp add: zero_option_def)
+  qed
+  thus ?thesis
+    unfolding to_signal2_def comp_def by auto
+qed
+
+theorem
+  assumes "b_simulate2 (Suc i) nand3 \<tau> res"
+  assumes "lookup (to_transaction2 \<tau> C) = 0"
+  shows "signal_of2 def res C (Suc i) \<longleftrightarrow> \<not> (signal_of2 False \<tau> A i \<and> signal_of2 False \<tau> B i)"
+proof (cases "lookup \<tau> 0 = 0")
+  case True
+  hence "init' 0 def_state {} 0 nand3 \<tau> = trans_post C True \<tau> 1" (is "_ = ?\<tau>'")
+    unfolding nand3_def by auto
+  hence ntime: "next_time 0 ?\<tau>' = 1"
+  proof -
+    have "?\<tau>' \<noteq> 0"
+      by (transfer', metis trans_post_raw_def map_upd_nonempty zero_map)
+    hence "next_time 0 ?\<tau>' = (LEAST n. dom (lookup ?\<tau>' n) \<noteq> {})"
+      unfolding next_time_def by auto
+    also have "... = 1"
+    proof (rule Least_equality)
+      show "dom (get_trans (trans_post C True \<tau> 1) 1) \<noteq> {}"
+        by (transfer', auto simp add: trans_post_raw_def)
+    next
+      { fix y :: nat
+        assume "y < 1"
+        hence "dom (get_trans (trans_post C True \<tau> 1) y) = {}"
+          using True by (transfer', simp add: trans_post_raw_def dom_def zero_map) }
+      thus "\<And>y. dom (get_trans (trans_post C True \<tau> 1) y) \<noteq> {} \<Longrightarrow> 1 \<le> y "
+        using le_less_linear by auto
+    qed
+    finally show "next_time 0 ?\<tau>' = 1"
+      by auto
+  qed
+  have ind1: "\<And>n. n < next_time 0 ?\<tau>' \<Longrightarrow> lookup ?\<tau>' n = 0"
+    using True unfolding `next_time 0 ?\<tau>' = 1` by (transfer', auto simp add: trans_post_raw_def)
+  have ind2: "\<And>s. s \<in> dom (lookup ?\<tau>' (next_time 0 ?\<tau>')) \<Longrightarrow>
+                        next_state 0 ?\<tau>' def_state s = the (lookup ?\<tau>' (next_time 0 ?\<tau>') s)"
+    unfolding next_state_def `next_time 0 ?\<tau>' = 1` Let_def by auto
+  have ind3: "\<And>n. next_time 0 ?\<tau>' \<le> n \<Longrightarrow> lookup (add_to_beh def_state 0 0 (next_time 0 ?\<tau>')) n = 0"
+    unfolding ntime add_to_beh_def by (transfer', auto)
+  have Cin: "C \<in> dom (lookup ?\<tau>' (next_time 0 ?\<tau>'))"
+    unfolding `next_time 0 ?\<tau>' = 1`  by (transfer', auto simp add: trans_post_raw_def)
+  { assume "A \<notin> next_event 0 ?\<tau>' def_state \<and> B \<notin> next_event 0 ?\<tau>' def_state"
+    hence "A \<notin> dom (lookup ?\<tau>' (next_time 0 ?\<tau>')) \<or> the (lookup ?\<tau>' (next_time 0 ?\<tau>') A) = False"
+      and "B \<notin> dom (lookup ?\<tau>' (next_time 0 ?\<tau>')) \<or> the (lookup ?\<tau>' (next_time 0 ?\<tau>') B) = False"
+      unfolding next_event_def ntime Let_def by auto
+    hence "True \<longleftrightarrow>  \<not> (next_state 0 ?\<tau>' def_state A \<and> next_state 0 ?\<tau>' def_state B)"
+      unfolding next_state_def ntime Let_def  by (simp add: override_on_def)
+    moreover have "next_state 0 ?\<tau>' def_state C = True"
+      using Cin unfolding next_state_def ntime Let_def  by (transfer', auto simp add: trans_post_raw_def)
+    ultimately have "next_state 0 ?\<tau>' def_state C \<longleftrightarrow>
+                                     \<not> (next_state 0 ?\<tau>' def_state A \<and> next_state 0 ?\<tau>' def_state B)"
+      by auto }
+  note ind4 = this
+  have ind5: "\<And>n. next_time 0 ?\<tau>' < n \<Longrightarrow> lookup (to_transaction2 ?\<tau>' C) n = 0"
+    unfolding ntime by (transfer', auto simp add: trans_post_raw_def to_trans_raw2_def zero_option_def)
+  hence bigstep: "(Suc i),
+         next_time 0 (trans_post C True \<tau> 1) ,
+         next_state 0 (trans_post C True \<tau> 1) def_state ,
+         next_event 0 (trans_post C True \<tau> 1) def_state ,
+         add_to_beh def_state empty_trans 0 (next_time 0 (trans_post C True \<tau> 1))
+      \<turnstile> <nand3 , trans_post C True \<tau> 1> \<leadsto> res"
+    using bsimulate2_obt_big_step[OF assms(1) `init' 0 def_state {} 0 nand3 \<tau> = ?\<tau>'`] by auto
+  have *: "1 \<le> i \<Longrightarrow>
+     signal_of2 def res C (Suc i) \<longleftrightarrow>
+  \<not> (signal_of2 (next_state 0 ?\<tau>' def_state A) ?\<tau>' A i \<and> signal_of2 (next_state 0 ?\<tau>' def_state B) ?\<tau>' B i)"
+    using nand3_correctness_ind[OF bigstep _ _ ind1 ind2 ind3 _ ind4 ind5] unfolding ntime by auto
+  moreover have "1 \<le> i \<Longrightarrow> signal_of2 (next_state 0 ?\<tau>' def_state A) ?\<tau>' A i = signal_of2 False ?\<tau>' A i"
+  proof (cases "inf_time (to_transaction2 ?\<tau>') A i = None")
+    case True
+    assume "1 \<le> i"
+    have "\<forall>k. k \<le> i \<longrightarrow> lookup (to_transaction2 ?\<tau>' A) k = 0"
+      using True by (auto dest!: inf_time_noneE2)
+    hence "lookup (to_transaction2 ?\<tau>' A) 1 = 0"
+      using `1 \<le> i` by auto
+    hence "A \<notin> dom (lookup ?\<tau>' 1)"
+      apply transfer' unfolding trans_post_raw_def to_trans_raw2_def
+      by (simp add: domIff zero_option_def)
+    have "signal_of2 (next_state 0 ?\<tau>' def_state A) ?\<tau>' A i = next_state 0 ?\<tau>' def_state A"
+      using True unfolding to_signal2_def comp_def by auto
+    also have "... = False"
+      using `A \<notin> dom (lookup ?\<tau>' 1)` unfolding next_state_def ntime Let_def by auto
+    finally have 0: "signal_of2 (next_state 0 ?\<tau>' def_state A) ?\<tau>' A i = False"
+      by auto
+    have 1: "signal_of2 False ?\<tau>' A i = False"
+      using True unfolding to_signal2_def comp_def by auto
+    then show ?thesis
+      using 0 1 by auto
+  next
+    case False
+    then obtain ta where "inf_time (to_transaction2 (trans_post C True \<tau> 1)) A i = Some ta"
+      by auto
+    then show ?thesis
+      unfolding to_signal2_def comp_def by auto
+  qed
+  moreover have "1 \<le> i \<Longrightarrow> signal_of2 (next_state 0 ?\<tau>' def_state B) ?\<tau>' B i = signal_of2 False ?\<tau>' B i"
+  proof (cases "inf_time (to_transaction2 ?\<tau>') B i = None")
+    case True
+    assume "1 \<le> i"
+    have "\<forall>k. k \<le> i \<longrightarrow> lookup (to_transaction2 ?\<tau>' B) k = 0"
+      using True by (auto dest!: inf_time_noneE2)
+    hence "lookup (to_transaction2 ?\<tau>' B) 1 = 0"
+      using `1 \<le> i` by auto
+    hence "B \<notin> dom (lookup ?\<tau>' 1)"
+      apply transfer' unfolding trans_post_raw_def to_trans_raw2_def
+      by (simp add: domIff zero_option_def)
+    have "signal_of2 (next_state 0 ?\<tau>' def_state B) ?\<tau>' B i = next_state 0 ?\<tau>' def_state B"
+      using True unfolding to_signal2_def comp_def by auto
+    also have "... = False"
+      using `B \<notin> dom (lookup ?\<tau>' 1)` unfolding next_state_def ntime Let_def by auto
+    finally have 0: "signal_of2 (next_state 0 ?\<tau>' def_state B) ?\<tau>' B i = False"
+      by auto
+    have 1: "signal_of2 False ?\<tau>' B i = False"
+      using True unfolding to_signal2_def comp_def by auto
+    then show ?thesis
+      using 0 1 by auto
+  next
+    case False
+    then obtain ta where "inf_time (to_transaction2 (trans_post C True \<tau> 1)) B i = Some ta"
+      by auto
+    then show ?thesis
+      unfolding to_signal2_def comp_def by auto
+  qed
+  ultimately have IR: "1 \<le> i \<Longrightarrow> signal_of2 def res C (Suc i) \<longleftrightarrow>
+                                            \<not> (signal_of2 False ?\<tau>' A i \<and> signal_of2 False ?\<tau>' B i)"
+    by auto
+  have "lookup ?\<tau>' 0 = 0"
+    using True by (transfer', simp add: trans_post_raw_def)
+  have "signal_of2 False ?\<tau>' A 0 = False"
+    using inf_time_at_zero[OF `lookup ?\<tau>' 0 = 0`] unfolding to_signal2_def comp_def by auto
+  have "signal_of2 False ?\<tau>' B 0 = False"
+    using inf_time_at_zero[OF `lookup ?\<tau>' 0 = 0`] unfolding to_signal2_def comp_def by auto
+  have "next_time 0 (trans_post C True \<tau> 1) \<le> Suc i"
+    unfolding ntime by auto
+  have "1 \<le> next_time 0 (trans_post C True \<tau> 1)"
+    unfolding ntime by auto
+  have "lookup res 1 = get_trans
+   (Poly_Mapping.update (next_time 0 (trans_post C True \<tau> 1)) (Some \<circ> next_state 0 (trans_post C True \<tau> 1) def_state)
+     (add_to_beh def_state empty_trans 0 (next_time 0 (trans_post C True \<tau> 1)))) 1"
+    using beh_res2[OF bigstep ind1 `next_time 0 (trans_post C True \<tau> 1) \<le> Suc i` _ ind2 ind3 `1 \<le> next_time 0 (trans_post C True \<tau> 1)`]
+    by auto
+  also have "... = lookup (Poly_Mapping.update 1 (Some o next_state 0 ?\<tau>' def_state) (add_to_beh def_state 0 0 1)) 1"
+    unfolding ntime by auto
+  also have "... = Some o next_state 0 ?\<tau>' def_state"
+    by (simp add: lookup_update)
+  finally have "lookup res 1  = Some o next_state 0 ?\<tau>' def_state"
+    by auto
+  hence "signal_of2 def res C 1 = next_state 0 ?\<tau>' def_state C"
+    using lookup_some_signal_of2[OF `lookup res 1 = Some o next_state 0 ?\<tau>' def_state`] by auto
+  also have "... = True"
+    unfolding next_state_def ntime Let_def by (transfer', auto simp add: trans_post_raw_def)
+  also have "... \<longleftrightarrow> \<not> (signal_of2 False ?\<tau>' A 0 \<and> signal_of2 False ?\<tau>' B 0)"
+    unfolding `signal_of2 False ?\<tau>' A 0 = False` `signal_of2 False ?\<tau>' B 0 = False` by auto
+  finally have IR0: "signal_of2 def res C 1 \<longleftrightarrow> \<not> (signal_of2 False ?\<tau>' A 0 \<and> signal_of2 False ?\<tau>' B 0)"
+    by auto
+
+  have "signal_of2 False ?\<tau>' A i = signal_of2 False \<tau> A i" and "signal_of2 False ?\<tau>' B i = signal_of2 False \<tau> B i"
+    using signal_of_trans_post   by (metis sig.distinct(3))(meson sig.simps(6) signal_of_trans_post)
+  thus ?thesis
+    using IR IR0  using le_less_linear by auto
+next
+  case False
+  hence "init' 0 def_state {} 0 nand3 \<tau> = trans_post C True \<tau> 1" (is "_ = ?\<tau>'")
+    unfolding nand3_def by auto
+  hence ntime: "next_time 0 ?\<tau>' = 0"
+  proof -
+    have "?\<tau>' \<noteq> 0"
+      by (transfer', metis trans_post_raw_def map_upd_nonempty zero_map)
+    hence "next_time 0 ?\<tau>' = (LEAST n. dom (lookup ?\<tau>' n) \<noteq> {})"
+      unfolding next_time_def by auto
+    also have "... = 0"
+    proof (rule Least_equality)
+      show "dom (get_trans (trans_post C True \<tau> 1) 0) \<noteq> {}"
+        using False by (transfer', auto simp add: trans_post_raw_def zero_fun_def zero_option_def)
+    next
+      { fix y :: nat
+        assume "y < 0"
+        hence "False" by auto
+        hence "dom (get_trans (trans_post C True \<tau> 1) y) = {}"
+          by auto }
+      thus "\<And>y. dom (get_trans (trans_post C True \<tau> 1) y) \<noteq> {} \<Longrightarrow> 0 \<le> y "
+        using le_less_linear by auto
+    qed
+    finally show "next_time 0 ?\<tau>' = 0"
+      by auto
+  qed
+
+  define t' where "t' = next_time 0 ?\<tau>'"
+  have t'_def': "t' = 0"
+  proof -
+    have "?\<tau>' \<noteq> 0"
+      apply transfer' unfolding trans_post_raw_def  by (metis map_upd_nonempty zero_map)
+    hence "next_time 0 ?\<tau>' = (LEAST n. dom (lookup ?\<tau>' n) \<noteq> {})"
+      unfolding next_time_def by auto
+    also have "... = 0"
+    proof (rule Least_equality)
+      show "dom (get_trans (trans_post C True \<tau> 1) 0) \<noteq> {}"
+        using False apply transfer' unfolding trans_post_raw_def zero_fun_def zero_option_def by auto
+    next
+      { fix y :: nat
+        assume "y < 0"
+        hence "False" by auto
+        hence "dom (get_trans (trans_post C True \<tau> 1) y) = {}" by auto }
+      thus "\<And>y. dom (get_trans (trans_post C True \<tau> 1) y) \<noteq> {} \<Longrightarrow> 0 \<le> y"
+        by auto
+    qed
+    finally have "next_time 0 ?\<tau>' = 0"
+      by auto
+    thus ?thesis
+      unfolding t'_def by auto
+  qed
+  hence ntime: "(next_time 0 (trans_post C True \<tau> 1)) = 0"
+    unfolding t'_def[THEN sym] by auto
+
+  define \<sigma>' where "\<sigma>' = next_state 0 ?\<tau>' def_state"
+  define \<gamma>' where "\<gamma>' = next_event 0 ?\<tau>' def_state"
+  define \<theta>' where "\<theta>' = add_to_beh def_state (0 :: sig transaction) 0 t'"
+  hence "\<theta>' = 0"
+    unfolding t'_def' add_to_beh_def by auto
+
+  hence bigstep: "(Suc i), t' , \<sigma>' , \<gamma>', \<theta>' \<turnstile> <nand3 , ?\<tau>'> \<leadsto> res"
+    using bsimulate2_obt_big_step[OF assms(1) `init' 0 def_state {} 0 nand3 \<tau> = ?\<tau>'`]
+    unfolding \<sigma>'_def \<gamma>'_def \<theta>'_def t'_def by auto
+  hence bigstep': "(Suc i), 0 , \<sigma>' , \<gamma>', 0 \<turnstile> <nand3 , ?\<tau>'> \<leadsto> res"
+    unfolding t'_def' `\<theta>' = 0` by auto
+  have "\<not> quiet ?\<tau>' \<gamma>'"
+    unfolding quiet_def apply transfer' unfolding trans_post_raw_def
+    by (metis map_upd_nonempty zero_map)
+  moreover have "0 \<le> Suc i"
+    by auto
+  obtain \<tau>'' where cyc: "0 , \<sigma>' , \<gamma>' , empty_trans \<turnstile> <nand3 , rem_curr_trans 0 ?\<tau>'> \<longrightarrow>\<^sub>c \<tau>''" and
+    bigstep'': "(Suc i), next_time 0 \<tau>'' , next_state 0 \<tau>'' \<sigma>' , next_event 0 \<tau>'' \<sigma>' , add_to_beh \<sigma>' empty_trans 0 (next_time 0 \<tau>'') \<turnstile> <nand3 , \<tau>''> \<leadsto> res"
+    using case_bau2[OF `0 \<le> Suc i` `\<not> quiet ?\<tau>' \<gamma>'` bigstep'] by auto
+  define \<sigma>'' where "\<sigma>'' = next_state 0 \<tau>'' \<sigma>'"
+  define \<gamma>'' where "\<gamma>'' = next_event 0 \<tau>'' \<sigma>'"
+  define \<theta>'' where "\<theta>'' = add_to_beh \<sigma>' 0 0 (next_time 0 \<tau>'')"
+  have bigstep3 : "(Suc i), next_time 0 \<tau>'' , \<sigma>'' , \<gamma>'' , \<theta>'' \<turnstile> <nand3 , \<tau>''> \<leadsto> res"
+    using bigstep'' unfolding \<sigma>''_def \<gamma>''_def \<theta>''_def by auto
+
+  have ind1: "\<And>n. n < next_time 0 ?\<tau>' \<Longrightarrow> lookup ?\<tau>' n = 0"
+    unfolding `next_time 0 ?\<tau>' = 0` by (transfer', auto simp add: trans_post_raw_def)
+  have ind1': "\<And>n. n < next_time 0 \<tau>'' \<Longrightarrow> lookup \<tau>'' n = 0"
+  proof (cases "\<tau>'' = 0")
+    case True
+    hence "next_time 0 \<tau>'' = 0"
+      by auto
+    { fix n
+      assume "n < next_time 0 \<tau>''"
+      hence "n < 0" unfolding `next_time 0 \<tau>'' = 0` by auto
+      hence "False" by auto
+      hence "lookup \<tau>'' n = 0" by auto }
+    then show "\<And>n. n < next_time 0 \<tau>'' \<Longrightarrow> lookup \<tau>'' n = 0" by auto
+  next
+    case False
+    hence "next_time 0 \<tau>'' = (LEAST n. dom (lookup \<tau>'' n) \<noteq> {})"
+      unfolding next_time_def by auto
+    then show "\<And>n. n < next_time 0 \<tau>'' \<Longrightarrow> lookup \<tau>'' n = 0"
+      using Least_le  next_time_at_least2 by blast
+  qed
+  have ind2: "\<And>s. s \<in> dom (lookup ?\<tau>' (next_time 0 ?\<tau>')) \<Longrightarrow>
+                        next_state 0 ?\<tau>' def_state s = the (lookup ?\<tau>' (next_time 0 ?\<tau>') s)"
+    unfolding next_state_def `next_time 0 ?\<tau>' = 0` Let_def by auto
+  have ind2': "\<And>s. s \<in> dom (lookup \<tau>'' (next_time 0 \<tau>'')) \<Longrightarrow>
+                        \<sigma>'' s = the (lookup \<tau>'' (next_time 0 \<tau>'') s)"
+    unfolding next_state_def Let_def \<sigma>''_def by auto
+  have ind3: "\<And>n. next_time 0 ?\<tau>' \<le> n \<Longrightarrow> lookup (add_to_beh def_state 0 0 (next_time 0 ?\<tau>')) n = 0"
+    unfolding ntime add_to_beh_def by (transfer', auto)
+  have ind3': "\<And>n. next_time 0 \<tau>'' \<le> n \<Longrightarrow> lookup \<theta>'' n = 0"
+    unfolding \<theta>''_def add_to_beh_def by transfer' auto
+  consider (either) "A \<in> \<gamma>' \<or> B \<in> \<gamma>'" | (none) "A \<notin> \<gamma>' \<and> B \<notin> \<gamma>'"
+    by auto
+  thus ?thesis
+  proof (cases)
+    case either
+    hence \<tau>''_def: "\<tau>'' = trans_post C (\<not> (\<sigma>' A \<and> \<sigma>' B)) (rem_curr_trans 0 ?\<tau>') 1"
+      using cyc unfolding nand3_def by auto
+    hence "\<tau>'' \<noteq> 0"
+      unfolding rem_curr_trans_def apply transfer' unfolding trans_post_raw_def
+      by (metis (no_types, lifting) fun_upd_same option.simps(3) zero_map)
+    hence "next_time 0 \<tau>'' = (LEAST n. dom (lookup \<tau>'' n) \<noteq> {})"
+      unfolding next_time_def by auto
+    also have "... = 1"
+    proof (rule Least_equality)
+      show "dom (get_trans \<tau>'' 1) \<noteq> {}"
+        unfolding \<tau>''_def rem_curr_trans_def apply transfer' unfolding trans_post_raw_def by auto
+    next
+      { fix y :: nat
+        assume "y < 1"
+        hence "y = 0" by auto
+        have "dom (get_trans \<tau>'' y) = {}" unfolding `y = 0` \<tau>''_def rem_curr_trans_def
+          apply transfer' unfolding trans_post_raw_def  by (simp add: dom_def zero_map) }
+      thus "\<And>y. dom (get_trans \<tau>'' y) \<noteq> {} \<Longrightarrow> 1 \<le> y "
+        using le_less_linear by auto
+    qed
+    finally have "next_time 0 \<tau>'' = 1"
+      by auto
+    { assume "A \<notin> next_event 0 \<tau>'' \<sigma>' \<and> B \<notin> next_event 0 \<tau>'' \<sigma>'"
+      hence "A \<notin> dom (lookup \<tau>'' (next_time 0 \<tau>'')) \<or> the (lookup \<tau>'' (next_time 0 \<tau>'') A) = \<sigma>' A"
+        and "B \<notin> dom (lookup \<tau>'' (next_time 0 \<tau>'')) \<or> the (lookup \<tau>'' (next_time 0 \<tau>'') B) = \<sigma>' B"
+        unfolding next_event_def ntime Let_def by auto
+      hence helper: "\<not> (\<sigma>' A \<and> \<sigma>' B) \<longleftrightarrow>  \<not> (next_state 0 \<tau>'' \<sigma>' A \<and> next_state 0 \<tau>'' \<sigma>' B)"
+        unfolding next_state_def Let_def  by (simp add: override_on_def)
+      have "next_state 0 \<tau>'' \<sigma>' C \<longleftrightarrow> (let m = get_trans \<tau>'' (next_time 0 \<tau>'') in override_on \<sigma>' (the \<circ> m) (dom m)) C"
+        unfolding next_state_def by auto
+      also have "... = (let m = get_trans \<tau>'' 1 in override_on \<sigma>' (the \<circ> m) (dom m)) C"
+        unfolding `next_time 0 \<tau>'' = 1` by auto
+      also have "... \<longleftrightarrow> \<not> (\<sigma>' A \<and> \<sigma>' B)"
+        unfolding \<tau>''_def rem_curr_trans_def apply transfer' unfolding trans_post_raw_def Let_def
+        by auto
+      finally have "next_state 0 \<tau>'' \<sigma>' C \<longleftrightarrow> \<not> (\<sigma>' A \<and> \<sigma>' B)"
+        by auto
+      hence "next_state 0 \<tau>'' \<sigma>' C \<longleftrightarrow> \<not> (next_state 0 \<tau>'' \<sigma>' A \<and> next_state 0 \<tau>'' \<sigma>' B)"
+        using helper by auto }
+    hence  ind4': "A \<notin> \<gamma>'' \<and> B \<notin> \<gamma>'' \<Longrightarrow> \<sigma>'' C = (\<not> (\<sigma>'' A \<and> \<sigma>'' B))"
+      unfolding \<gamma>''_def \<sigma>''_def by auto
+    have "\<And>n. 1 < n \<Longrightarrow> lookup (to_transaction2 \<tau>'' C) n = 0"
+      unfolding \<tau>''_def rem_curr_trans_def apply transfer' unfolding trans_post_raw_def to_trans_raw2_def
+      by (simp add: zero_option_def)
+    hence ind5': "\<And>n. next_time 0 \<tau>'' < n \<Longrightarrow> lookup (to_transaction2 \<tau>'' C) n = 0"
+      unfolding `next_time 0 \<tau>'' = 1` by auto
+    have *: "1 \<le> i \<Longrightarrow>
+       signal_of2 def res C (Suc i) = (\<not> (signal_of2 (\<sigma>'' A) \<tau>'' A i \<and> signal_of2 (\<sigma>'' B) \<tau>'' B i))"
+      using nand3_correctness_ind[OF bigstep3 _ _ ind1' ind2' ind3' _ ind4' ind5']
+      unfolding `next_time 0 \<tau>'' = 1` by auto
+    moreover have "1 \<le> i \<Longrightarrow> signal_of2 (\<sigma>'' A) \<tau>'' A i = signal_of2 (\<sigma>' A) \<tau>'' A i"
+    proof (cases "inf_time (to_transaction2 \<tau>'') A i = None")
+      case True
+      assume "1 \<le> i"
+      have "\<forall>k. k \<le> i \<longrightarrow> lookup (to_transaction2 \<tau>'' A) k = 0"
+        using True by (auto dest!: inf_time_noneE2)
+      hence "lookup (to_transaction2 \<tau>'' A) 1 = 0"
+        using `1 \<le> i` by auto
+      hence "A \<notin> dom (lookup \<tau>'' 1)"
+        apply transfer' unfolding trans_post_raw_def to_trans_raw2_def
+        by (simp add: domIff zero_option_def)
+      have "signal_of2 (\<sigma>'' A) \<tau>'' A i = next_state 0 \<tau>'' \<sigma>' A"
+        using True unfolding to_signal2_def comp_def \<tau>''_def  by (simp add: \<sigma>''_def \<tau>''_def)
+      also have "... = \<sigma>' A"
+        using `A \<notin> dom (lookup \<tau>'' 1)` unfolding next_state_def
+        by (metis \<open>next_time 0 \<tau>'' = 1\<close> override_on_apply_notin)
+      finally have 0: "signal_of2 (\<sigma>'' A) \<tau>'' A i = \<sigma>' A"
+        by auto
+      have 1: "signal_of2 (\<sigma>' A) \<tau>'' A i = \<sigma>' A"
+        using True unfolding to_signal2_def comp_def by auto
+      then show ?thesis
+        using 0 1 by auto
+    next
+      case False
+      then obtain ta where "inf_time (to_transaction2 \<tau>'') A i = Some ta"
+        by auto
+      then show ?thesis
+        unfolding to_signal2_def comp_def by auto
+    qed
+    moreover have "1 \<le> i \<Longrightarrow> signal_of2 (\<sigma>'' B) \<tau>'' B i = signal_of2 (\<sigma>' B) \<tau>'' B i"
+    proof (cases "inf_time (to_transaction2 \<tau>'') B i = None")
+      case True
+      assume "1 \<le> i"
+      have "\<forall>k. k \<le> i \<longrightarrow> lookup (to_transaction2 \<tau>'' B) k = 0"
+        using True by (auto dest!: inf_time_noneE2)
+      hence "lookup (to_transaction2 \<tau>'' B) 1 = 0"
+        using `1 \<le> i` by auto
+      hence "B \<notin> dom (lookup \<tau>'' 1)"
+        apply transfer' unfolding trans_post_raw_def to_trans_raw2_def
+        by (simp add: domIff zero_option_def)
+      have "signal_of2 (\<sigma>'' B) \<tau>'' B i = next_state 0 \<tau>'' \<sigma>' B"
+        using True unfolding to_signal2_def comp_def \<tau>''_def  by (simp add: \<sigma>''_def \<tau>''_def)
+      also have "... = \<sigma>' B"
+        using `B \<notin> dom (lookup \<tau>'' 1)` unfolding next_state_def
+        by (metis \<open>next_time 0 \<tau>'' = 1\<close> override_on_apply_notin)
+      finally have 0: "signal_of2 (\<sigma>'' B) \<tau>'' B i = \<sigma>' B"
+        by auto
+      have 1: "signal_of2 (\<sigma>' B) \<tau>'' B i = \<sigma>' B"
+        using True unfolding to_signal2_def comp_def by auto
+      then show ?thesis
+        using 0 1 by auto
+    next
+      case False
+      then obtain ta where "inf_time (to_transaction2 \<tau>'') B i = Some ta"
+        by auto
+      then show ?thesis
+        unfolding to_signal2_def comp_def by auto
+    qed
+    ultimately have IR: "1 \<le> i \<Longrightarrow> signal_of2 def res C (Suc i) \<longleftrightarrow>
+                                          \<not> (signal_of2 (\<sigma>' A) \<tau>'' A i \<and> signal_of2 (\<sigma>' B) \<tau>'' B i)"
+      by auto
+    have "lookup \<tau>'' 0 = 0"
+      unfolding \<tau>''_def rem_curr_trans_def by (transfer', auto simp add: trans_post_raw_def)
+    have sA: "signal_of2 (\<sigma>' A) \<tau>'' A 0 = \<sigma>' A"
+      using inf_time_at_zero[OF `lookup \<tau>'' 0 = 0`] unfolding to_signal2_def comp_def by auto
+    have sB: "signal_of2 (\<sigma>' B) \<tau>'' B 0 = \<sigma>' B"
+      using inf_time_at_zero[OF `lookup \<tau>'' 0 = 0`] unfolding to_signal2_def comp_def by auto
+    have "next_time 0 \<tau>'' \<le> Suc i" and "1 \<le> next_time 0 \<tau>''"
+      unfolding `next_time 0 \<tau>'' = 1` by auto
+    have "get_trans res 1 = get_trans (Poly_Mapping.update 1 (Some \<circ> \<sigma>'') \<theta>'') 1"
+      using beh_res2[OF bigstep3 ind1' `next_time 0 \<tau>'' \<le> Suc i` _ ind2' ind3' `1 \<le> next_time 0 \<tau>''`]
+      unfolding `next_time 0 \<tau>'' = 1` by auto
+    also have "... = Some o \<sigma>''"
+      by (simp add: lookup_update)
+    finally have "lookup res 1  = Some o \<sigma>''"
+      by auto
+    hence "signal_of2 def res C 1 = \<sigma>'' C"
+      using lookup_some_signal_of2[OF `lookup res 1 =Some o \<sigma>''`] by auto
+    also have "... \<longleftrightarrow> (let m = get_trans \<tau>'' 1 in override_on \<sigma>' (the \<circ> m) (dom m)) C"
+      unfolding \<sigma>''_def next_state_def `next_time 0 \<tau>'' = 1` by auto
+    also have "... \<longleftrightarrow> \<not> (\<sigma>' A \<and> \<sigma>' B)"
+      unfolding \<tau>''_def Let_def rem_curr_trans_def apply transfer'  unfolding trans_post_raw_def
+      by auto
+    also have "... \<longleftrightarrow> \<not> (signal_of2 (\<sigma>' A) \<tau>'' A 0 \<and> signal_of2 (\<sigma>' B) \<tau>'' B 0)"
+      using sA sB by auto
+    finally have IR0: "signal_of2 def res C 1 \<longleftrightarrow> \<not> (signal_of2 (\<sigma>' A) \<tau>'' A 0 \<and> signal_of2 (\<sigma>' B) \<tau>'' B 0)"
+      by auto
+
+    have "signal_of2 (\<sigma>' A) \<tau>'' A i = signal_of2 (\<sigma>' A) (rem_curr_trans 0 ?\<tau>') A i"
+      using signal_of_trans_post unfolding \<tau>''_def by (metis \<tau>''_def sig.distinct(3))
+    also have "... = signal_of2 (\<sigma>' A) ?\<tau>' A i"
+      using signal_of2_rem_curr_trans_at_0 ind2 unfolding ntime \<sigma>'_def  by metis
+    also have "... = signal_of2 (\<sigma>' A) \<tau> A i"
+      using signal_of_trans_post  by (metis sig.distinct(3))
+    also have "... = signal_of2 False \<tau> A i"
+    proof -
+      have "lookup (to_transaction2 \<tau> A) 0 \<noteq> None \<or> lookup (to_transaction2 \<tau> A) 0 = None"
+        by auto
+      moreover
+      { assume "lookup (to_transaction2 \<tau> A) 0 \<noteq> None"
+        with signal_of2_cong_neq_none_at_0 have ?thesis by metis }
+      moreover
+      { assume "lookup (to_transaction2 \<tau> A) 0 = None"
+        hence "A \<notin> dom (get_trans (trans_post C True \<tau> 1) 0)"
+          apply transfer' unfolding to_trans_raw2_def trans_post_raw_def by auto
+        hence "\<sigma>' A = False"
+          unfolding \<sigma>'_def next_state_def `next_time 0 ?\<tau>' = 0` Let_def by auto
+        hence ?thesis by auto }
+      ultimately show ?thesis by auto
+    qed
+    finally have hel: "signal_of2 (\<sigma>' A) \<tau>'' A i = signal_of2 False \<tau> A i"
+      by auto
+
+    have "signal_of2 (\<sigma>' B) \<tau>'' B i = signal_of2 (\<sigma>' B) (rem_curr_trans 0 ?\<tau>') B i"
+      using signal_of_trans_post unfolding \<tau>''_def  by fastforce
+    also have "... = signal_of2 (\<sigma>' B) ?\<tau>' B i"
+      using signal_of2_rem_curr_trans_at_0 ind2 unfolding ntime \<sigma>'_def  by metis
+    also have "... = signal_of2 (\<sigma>' B) \<tau> B i"
+      using signal_of_trans_post   by fastforce
+    also have "... = signal_of2 False \<tau> B i"
+    proof -
+      have "lookup (to_transaction2 \<tau> B) 0 \<noteq> None \<or> lookup (to_transaction2 \<tau> B) 0 = None"
+        by auto
+      moreover
+      { assume "lookup (to_transaction2 \<tau> B) 0 \<noteq> None"
+        with signal_of2_cong_neq_none_at_0 have ?thesis by metis }
+      moreover
+      { assume "lookup (to_transaction2 \<tau> B) 0 = None"
+        hence "B \<notin> dom (get_trans (trans_post C True \<tau> 1) 0)"
+          apply transfer' unfolding to_trans_raw2_def trans_post_raw_def by auto
+        hence "\<sigma>' B = False"
+          unfolding \<sigma>'_def next_state_def `next_time 0 ?\<tau>' = 0` Let_def by auto
+        hence ?thesis by auto }
+      ultimately show ?thesis by auto
+    qed
+    finally have "signal_of2 (\<sigma>' B) \<tau>'' B i = signal_of2 False \<tau> B i"
+      by auto
+    then show ?thesis
+      using IR IR0 hel le_less_linear by auto
+  next
+    case none
+    hence \<tau>''_def: "\<tau>'' = rem_curr_trans 0 ?\<tau>'"
+      using cyc unfolding nand3_def by auto
+    hence "\<tau>'' \<noteq> 0"
+      unfolding rem_curr_trans_def apply transfer' unfolding trans_post_raw_def
+    proof -
+      fix \<tau>''' :: "nat \<Rightarrow> sig \<Rightarrow> bool option" and \<tau>' :: "nat \<Rightarrow> sig \<Rightarrow> bool option"
+      assume a1: "\<tau>''' = (\<lambda>t'. if t' = 1 then \<tau>' t'(C \<mapsto> True) else if 1 < t' then (\<tau>' t')(C := None) else \<tau>' t') (0 := 0)"
+      have "\<tau>' 1(C \<mapsto> True) = ((\<lambda>n. if n = 1 then \<tau>' n(C \<mapsto> True) else if 1 < n then (\<tau>' n)(C := None) else \<tau>' n) (0 := 0)) 1"
+        by simp
+      then show "\<tau>''' \<noteq> (\<lambda>n. 0)"
+        using a1 by (metis (no_types) fun_upd_same option.distinct(1) zero_map)
+    qed
+    hence "next_time 0 \<tau>'' = (LEAST n. dom (lookup \<tau>'' n) \<noteq> {})"
+      unfolding next_time_def by auto
+    also have "... = 1"
+    proof (rule Least_equality)
+      show "dom (get_trans \<tau>'' 1) \<noteq> {}"
+        unfolding \<tau>''_def unfolding rem_curr_trans_def by (transfer', auto simp add: trans_post_raw_def)
+    next
+      { fix y :: nat
+        assume "\<not> 1 \<le> y"
+        hence "y < 1" by auto hence "y = 0" by auto
+        hence "dom (get_trans \<tau>'' y) = {}"
+          unfolding \<tau>''_def rem_curr_trans_def apply transfer' by (auto simp add: trans_post_raw_def zero_map) }
+      thus "\<And>y. dom (get_trans \<tau>'' y) \<noteq> {} \<Longrightarrow> 1 \<le> y "
+        by auto
+    qed
+    finally have "next_time 0 \<tau>'' = 1"
+      by auto
+    have "\<sigma>' A = False" and "\<sigma>' B = False"
+      using none unfolding \<gamma>'_def \<sigma>'_def next_event_def Let_def ntime
+      by (metis \<gamma>'_def next_state_fixed_point none)+
+    { assume "A \<notin> next_event 0 \<tau>'' \<sigma>' \<and> B \<notin> next_event 0 \<tau>'' \<sigma>'"
+      hence "A \<notin> dom (lookup \<tau>'' (next_time 0 \<tau>'')) \<or> the (lookup \<tau>'' (next_time 0 \<tau>'') A) = \<sigma>' A"
+        and "B \<notin> dom (lookup \<tau>'' (next_time 0 \<tau>'')) \<or> the (lookup \<tau>'' (next_time 0 \<tau>'') B) = \<sigma>' B"
+        unfolding next_event_def ntime Let_def by auto
+      hence helper: "\<not> (\<sigma>' A \<and> \<sigma>' B) \<longleftrightarrow>  \<not> (next_state 0 \<tau>'' \<sigma>' A \<and> next_state 0 \<tau>'' \<sigma>' B)"
+        unfolding next_state_def Let_def  by (simp add: override_on_def)
+      have "next_state 0 \<tau>'' \<sigma>' C \<longleftrightarrow> (let m = get_trans \<tau>'' (next_time 0 \<tau>'') in override_on \<sigma>' (the \<circ> m) (dom m)) C"
+        unfolding next_state_def by auto
+      also have "... = (let m = get_trans \<tau>'' 1 in override_on \<sigma>' (the \<circ> m) (dom m)) C"
+        unfolding `next_time 0 \<tau>'' = 1` by auto
+      also have "... \<longleftrightarrow> \<not> (\<sigma>' A \<and> \<sigma>' B)"
+        unfolding \<tau>''_def rem_curr_trans_def `\<sigma>' A = False` `\<sigma>' B = False` apply transfer'
+        unfolding trans_post_raw_def Let_def by auto
+      finally have "next_state 0 \<tau>'' \<sigma>' C \<longleftrightarrow> \<not> (\<sigma>' A \<and> \<sigma>' B)"
+        by auto
+      hence "next_state 0 \<tau>'' \<sigma>' C \<longleftrightarrow> \<not> (next_state 0 \<tau>'' \<sigma>' A \<and> next_state 0 \<tau>'' \<sigma>' B)"
+        using helper by auto }
+    hence  ind4': "A \<notin> \<gamma>'' \<and> B \<notin> \<gamma>'' \<Longrightarrow> \<sigma>'' C = (\<not> (\<sigma>'' A \<and> \<sigma>'' B))"
+      unfolding \<gamma>''_def \<sigma>''_def by auto
+    have "\<And>n. 1 < n \<Longrightarrow> lookup (to_transaction2 \<tau>'' C) n = 0"
+      unfolding \<tau>''_def rem_curr_trans_def apply transfer' unfolding trans_post_raw_def to_trans_raw2_def
+      by (simp add: zero_option_def)
+    hence ind5': "\<And>n. next_time 0 \<tau>'' < n \<Longrightarrow> lookup (to_transaction2 \<tau>'' C) n = 0"
+      unfolding `next_time 0 \<tau>'' = 1` by auto
+    have *: "1 \<le> i \<Longrightarrow>
+       signal_of2 def res C (Suc i) = (\<not> (signal_of2 (\<sigma>'' A) \<tau>'' A i \<and> signal_of2 (\<sigma>'' B) \<tau>'' B i))"
+      using nand3_correctness_ind[OF bigstep3 _ _ ind1' ind2' ind3' _ ind4' ind5']
+      unfolding `next_time 0 \<tau>'' = 1` by auto
+    moreover have "1 \<le> i \<Longrightarrow> signal_of2 (\<sigma>'' A) \<tau>'' A i = signal_of2 (\<sigma>' A) \<tau>'' A i"
+    proof (cases "inf_time (to_transaction2 \<tau>'') A i = None")
+      case True
+      assume "1 \<le> i"
+      have "\<forall>k. k \<le> i \<longrightarrow> lookup (to_transaction2 \<tau>'' A) k = 0"
+        using True by (auto dest!: inf_time_noneE2)
+      hence "lookup (to_transaction2 \<tau>'' A) 1 = 0"
+        using `1 \<le> i` by auto
+      hence "A \<notin> dom (lookup \<tau>'' 1)"
+        apply transfer' unfolding trans_post_raw_def to_trans_raw2_def
+        by (simp add: domIff zero_option_def)
+      have "signal_of2 (\<sigma>'' A) \<tau>'' A i = next_state 0 \<tau>'' \<sigma>' A"
+        using True unfolding to_signal2_def comp_def \<tau>''_def  by (simp add: \<sigma>''_def \<tau>''_def)
+      also have "... = \<sigma>' A"
+        using `A \<notin> dom (lookup \<tau>'' 1)` unfolding next_state_def
+        by (metis \<open>next_time 0 \<tau>'' = 1\<close> override_on_apply_notin)
+      finally have 0: "signal_of2 (\<sigma>'' A) \<tau>'' A i = \<sigma>' A"
+        by auto
+      have 1: "signal_of2 (\<sigma>' A) \<tau>'' A i = \<sigma>' A"
+        using True unfolding to_signal2_def comp_def by auto
+      then show ?thesis
+        using 0 1 by auto
+    next
+      case False
+      then obtain ta where "inf_time (to_transaction2 \<tau>'') A i = Some ta"
+        by auto
+      then show ?thesis
+        unfolding to_signal2_def comp_def by auto
+    qed
+    moreover have "1 \<le> i \<Longrightarrow> signal_of2 (\<sigma>'' B) \<tau>'' B i = signal_of2 (\<sigma>' B) \<tau>'' B i"
+    proof (cases "inf_time (to_transaction2 \<tau>'') B i = None")
+      case True
+      assume "1 \<le> i"
+      have "\<forall>k. k \<le> i \<longrightarrow> lookup (to_transaction2 \<tau>'' B) k = 0"
+        using True by (auto dest!: inf_time_noneE2)
+      hence "lookup (to_transaction2 \<tau>'' B) 1 = 0"
+        using `1 \<le> i` by auto
+      hence "B \<notin> dom (lookup \<tau>'' 1)"
+        apply transfer' unfolding trans_post_raw_def to_trans_raw2_def
+        by (simp add: domIff zero_option_def)
+      have "signal_of2 (\<sigma>'' B) \<tau>'' B i = next_state 0 \<tau>'' \<sigma>' B"
+        using True unfolding to_signal2_def comp_def \<tau>''_def  by (simp add: \<sigma>''_def \<tau>''_def)
+      also have "... = \<sigma>' B"
+        using `B \<notin> dom (lookup \<tau>'' 1)` unfolding next_state_def
+        by (metis \<open>next_time 0 \<tau>'' = 1\<close> override_on_apply_notin)
+      finally have 0: "signal_of2 (\<sigma>'' B) \<tau>'' B i = \<sigma>' B"
+        by auto
+      have 1: "signal_of2 (\<sigma>' B) \<tau>'' B i = \<sigma>' B"
+        using True unfolding to_signal2_def comp_def by auto
+      then show ?thesis
+        using 0 1 by auto
+    next
+      case False
+      then obtain ta where "inf_time (to_transaction2 \<tau>'') B i = Some ta"
+        by auto
+      then show ?thesis
+        unfolding to_signal2_def comp_def by auto
+    qed
+    ultimately have IR: "1 \<le> i \<Longrightarrow> signal_of2 def res C (Suc i) \<longleftrightarrow>
+                                          \<not> (signal_of2 (\<sigma>' A) \<tau>'' A i \<and> signal_of2 (\<sigma>' B) \<tau>'' B i)"
+      by auto
+    have "lookup \<tau>'' 0 = 0"
+      unfolding \<tau>''_def rem_curr_trans_def by (transfer', auto simp add: trans_post_raw_def)
+    have sA: "signal_of2 (\<sigma>' A) \<tau>'' A 0 = \<sigma>' A"
+      using inf_time_at_zero[OF `lookup \<tau>'' 0 = 0`] unfolding to_signal2_def comp_def by auto
+    have sB: "signal_of2 (\<sigma>' B) \<tau>'' B 0 = \<sigma>' B"
+      using inf_time_at_zero[OF `lookup \<tau>'' 0 = 0`] unfolding to_signal2_def comp_def by auto
+    have "next_time 0 \<tau>'' \<le> Suc i" and "1 \<le> next_time 0 \<tau>''"
+      unfolding `next_time 0 \<tau>'' = 1` by auto
+    have "get_trans res 1 = get_trans (Poly_Mapping.update 1 (Some \<circ> \<sigma>'') \<theta>'') 1"
+      using beh_res2[OF bigstep3 ind1' `next_time 0 \<tau>'' \<le> Suc i` _ ind2' ind3' `1 \<le> next_time 0 \<tau>''`]
+      unfolding `next_time 0 \<tau>'' = 1` by auto
+    also have "... = Some o \<sigma>''"
+      by (simp add: lookup_update)
+    finally have "lookup res 1  = Some o \<sigma>''"
+      by auto
+    hence "signal_of2 def res C 1 = \<sigma>'' C"
+      using lookup_some_signal_of2[OF `lookup res 1 =Some o \<sigma>''`] by auto
+    also have "... \<longleftrightarrow> (let m = get_trans \<tau>'' 1 in override_on \<sigma>' (the \<circ> m) (dom m)) C"
+      unfolding \<sigma>''_def next_state_def `next_time 0 \<tau>'' = 1` by auto
+    also have "... \<longleftrightarrow> \<not> (\<sigma>' A \<and> \<sigma>' B)"
+      unfolding \<tau>''_def Let_def rem_curr_trans_def unfolding `\<sigma>' A = False` `\<sigma>' B = False`
+      apply transfer'  unfolding trans_post_raw_def  by auto
+    also have "... \<longleftrightarrow> \<not> (signal_of2 (\<sigma>' A) \<tau>'' A 0 \<and> signal_of2 (\<sigma>' B) \<tau>'' B 0)"
+      using sA sB by auto
+    finally have IR0: "signal_of2 def res C 1 \<longleftrightarrow> \<not> (signal_of2 (\<sigma>' A) \<tau>'' A 0 \<and> signal_of2 (\<sigma>' B) \<tau>'' B 0)"
+      by auto
+
+    have "signal_of2 (\<sigma>' A) \<tau>'' A i = signal_of2 (\<sigma>' A) (rem_curr_trans 0 ?\<tau>') A i"
+      using signal_of_trans_post unfolding \<tau>''_def by (metis \<tau>''_def sig.distinct(3))
+    also have "... = signal_of2 (\<sigma>' A) ?\<tau>' A i"
+      using signal_of2_rem_curr_trans_at_0 ind2 unfolding ntime \<sigma>'_def  by metis
+    also have "... = signal_of2 (\<sigma>' A) \<tau> A i"
+      using signal_of_trans_post  by (metis sig.distinct(3))
+    also have "... = signal_of2 False \<tau> A i"
+    proof -
+      have "lookup (to_transaction2 \<tau> A) 0 \<noteq> None \<or> lookup (to_transaction2 \<tau> A) 0 = None"
+        by auto
+      moreover
+      { assume "lookup (to_transaction2 \<tau> A) 0 \<noteq> None"
+        with signal_of2_cong_neq_none_at_0 have ?thesis by metis }
+      moreover
+      { assume "lookup (to_transaction2 \<tau> A) 0 = None"
+        hence "A \<notin> dom (get_trans (trans_post C True \<tau> 1) 0)"
+          apply transfer' unfolding to_trans_raw2_def trans_post_raw_def by auto
+        hence "\<sigma>' A = False"
+          unfolding \<sigma>'_def next_state_def `next_time 0 ?\<tau>' = 0` Let_def by auto
+        hence ?thesis by auto }
+      ultimately show ?thesis by auto
+    qed
+    finally have hel: "signal_of2 (\<sigma>' A) \<tau>'' A i = signal_of2 False \<tau> A i"
+      by auto
+    have "signal_of2 (\<sigma>' B) \<tau>'' B i = signal_of2 (\<sigma>' B) (rem_curr_trans 0 ?\<tau>') B i"
+      using signal_of_trans_post unfolding \<tau>''_def  by fastforce
+    also have "... = signal_of2 (\<sigma>' B) ?\<tau>' B i"
+      using signal_of2_rem_curr_trans_at_0 ind2 unfolding ntime \<sigma>'_def  by metis
+    also have "... = signal_of2 (\<sigma>' B) \<tau> B i"
+      using signal_of_trans_post   by fastforce
+    also have "... = signal_of2 False \<tau> B i"
+    proof -
+      have "lookup (to_transaction2 \<tau> B) 0 \<noteq> None \<or> lookup (to_transaction2 \<tau> B) 0 = None"
+        by auto
+      moreover
+      { assume "lookup (to_transaction2 \<tau> B) 0 \<noteq> None"
+        with signal_of2_cong_neq_none_at_0 have ?thesis by metis }
+      moreover
+      { assume "lookup (to_transaction2 \<tau> B) 0 = None"
+        hence "B \<notin> dom (get_trans (trans_post C True \<tau> 1) 0)"
+          apply transfer' unfolding to_trans_raw2_def trans_post_raw_def by auto
+        hence "\<sigma>' B = False"
+          unfolding \<sigma>'_def next_state_def `next_time 0 ?\<tau>' = 0` Let_def by auto
+        hence ?thesis by auto }
+      ultimately show ?thesis by auto
+    qed
+    finally have "signal_of2 (\<sigma>' B) \<tau>'' B i = signal_of2 False \<tau> B i"
+      by auto
+    then show ?thesis
+      using IR IR0 hel le_less_linear by auto
+  qed
+qed
+
 end
